subreadwrite

proof/amd64/common/Keccak1600_subreadwrite.ec
@@ -15,36 +15,30 @@ import IntOrder.
 
 (* MOVE TO SOMEWHERE ELSE? *)
 
-op bytes_at size cur at l=
- take size (drop cur (nseq at W8.zero++l)++nseq size W8.zero).
 
-
-lemma size_bytes_at sz cur at l:
- 0 <= sz =>
- size (bytes_at sz cur at l) = sz.
+(* get rid of unnecessary hypothesis *)
+lemma size_drop' ['a] n (s: 'a list):
+ size (drop n s) = max 0 (size s - max 0 n).
 proof.
-move=> Hsz; rewrite size_take // size_cat size_nseq ler_maxr //.
+case: (0 <= n) => H.
+ rewrite size_drop //; congr; congr.
+ by rewrite ler_maxr.
+rewrite (ler_maxl 0 n) 1:/# /=.
+rewrite drop_le0 1:/#.
 smt(size_ge0).
 qed.
 
-lemma size_bytes_at' sz cur at l:
- size (bytes_at sz cur at l) = max 0 sz.
+lemma size_memread':
+  forall (mem : global_mem_t) (a : address) (sz : int),
+    size (memread mem a sz) = max 0 sz.
 proof.
-case: (0 <= sz) => ?.
- by rewrite size_bytes_at // ler_maxr.
-by rewrite /bytes_at take_le0 /#.
+move=> m a sz; case: (0<=sz) => H.
+ by rewrite size_memread /#.
+by rewrite /memread mkseq0_le /#.
 qed.
 
-lemma bytes_at_zeros n cur at:
- 0 <= cur =>
- bytes_at n cur at [W8.zero] = u8zeros n.
-proof.
-move=> *.
-apply (eq_from_nth W8.zero).
- by rewrite size_bytes_at' size_nseq /#.
-move=> i; rewrite size_bytes_at' // => Hi.
-by rewrite nth_take 1..2:/# nth_cat ?size_drop 1:/# nth_drop 1..2:/# nth_cat !nth_u8zeros /#.
-qed.
+
+
 
 lemma get_u256bytes i w:
  (u256bytes w).[i] = w \bits8 i.
@@ -75,6 +69,10 @@ rewrite bits8E nth_out ?size_to_list //.
 apply W8.ext_eq => k Hk.
 by rewrite zerowE initiE //= get_out /#.
 qed.
+
+lemma u64bytes_or w1 w2 i:
+(u64bytes (w1 `|` w2)).[i] = (u64bytes w1).[i] `|` (u64bytes w2).[i].
+proof. by rewrite !nth_to_list orb8E. qed.
 
 lemma bits8_u64_shl8 (w: W64.t) k i:
  0 <= i < 8 =>
@@ -162,7 +160,10 @@ lemma zeroextu256_zero:
  zeroextu256 W128.zero = W256.zero
 by circuit.
 
-(* *)
+
+
+
+(** SHIFT operations *)
 
 lemma u64_shl0 (w: W64.t): w `<<<` 0 = w.
 proof. by apply W64.wordP => i Hi; rewrite shlwE Hi /=. qed.
@@ -243,6 +244,606 @@ phoare SHLQ_256_ph _w _sh:
 proof. by conseq SHLQ_256_ll (SHLQ_256_h _w _sh). qed.
 
 
+(**
+
+  Abstract specification of subread/subwrite acting on lists of bytes.
+
+ remark: these specifications shall later be instantiated into memory and array
+ read/writes.
+*)
+
+op u8prefAt (lw: bytes) off (l: bytes) =
+ forall i,
+  lw.[i] = if (max 0 off) <= i < size lw
+           then l.[i-max 0 off]
+           else W8.zero.
+
+lemma u8prefAt0 lw cur at l n:
+ u8prefAt lw (at - cur) l =>
+ cur + size lw <= at \/ l = u8zeros n =>
+ lw = u8zeros (size lw).
+proof.
+move => H [H1|Hl]; apply (eq_from_nth W8.zero);
+ 1,3:(by rewrite size_nseq; smt(size_ge0));
+ move => i Hi; rewrite H nth_u8zeros;
+ case: (max 0 (at-cur) <= i) => C //=; rewrite ifT 1:/#.
+ by rewrite nth_out ?size_rcons //; smt(size_ge0). 
+by rewrite Hl nth_u8zeros.
+qed.
+
+lemma nth_u64bytes_shl l w k i:
+ 0 <= k =>
+ u8prefAt (u64bytes w) 0 l =>
+ (u64bytes (w `<<<` 8 * k)).[i]
+ = if k <= i < 8 then l.[i - k] else W8.zero.
+proof.
+move=> Hk H.
+case: (0 <= i < 8) => Hi; last first.
+ by rewrite nth_out ?size_to_list /#.
+rewrite nth_to_list bits8_u64_shl8 // -nth_to_list H ler_maxr //=.
+by rewrite size_to_list; smt(nth_out).
+qed.
+
+abbrev u8prefAbsorb (lw: bytes) off (l: bytes) tb =
+ u8prefAt lw off (rcons l (of_int tb)).
+
+lemma u8prefAbsorbP lw off l tb:
+ u8prefAbsorb lw off l tb <=>
+ forall i,
+  lw.[i] = if (max 0 off) <= i < size lw
+           then if i-max 0 off = size l
+                then W8.of_int tb
+                else l.[i-max 0 off]
+           else W8.zero.
+proof. smt(nth_rcons nth_out). qed.
+
+lemma u8prefAbsorb0 lw cur at l tb:
+ u8prefAbsorb lw (at - cur) l tb =>
+ cur + size lw <= at \/ l=[] /\ tb=0 =>
+ lw = u8zeros (size lw).
+proof.
+move=> /u8prefAt0 H [H1|[E1 E2]]; apply (H 1); first smt().
+by right; rewrite -cats1 E1 E2 /= nseq1.
+qed.
+
+op srincr sz (cur at len:int) =
+ if 0 <= at-cur < sz
+ then min (max 0 len) (cur+sz-at)
+ else 0.
+
+lemma srincr_out sz cur at l:
+ ! 0 <= at-cur < sz => srincr sz cur at l = 0
+by smt().
+
+op srfnsh sz (cur at len tb:int) =
+ if 0 <= at-cur < sz
+ then 0 <= len /\ at+len < cur+sz /\ tb<>0
+ else false.
+
+abbrev srat sz cur at len tb =
+ at + srincr sz cur at len + b2i (srfnsh sz cur at len tb).
+abbrev srtb sz cur at len tb =
+ if srfnsh sz cur at len tb then 0 else tb.
+abbrev srl sz cur at (l:W8.t list) =
+ drop (srincr sz cur at (size l)) l.
+abbrev srlen sz cur at len =
+ len-(srincr sz cur at len).
+
+lemma srincr0 sz cur at:
+ srincr sz cur at 0 = 0
+by smt().
+lemma srtb0 sz cur at:
+ srtb sz cur at 0 0 = 0
+by smt().
+lemma srl0 sz cur at:
+ srl sz cur at [] = []
+by smt().
+lemma srat0 sz cur at:
+ srat sz cur at 0 0 = at
+by smt().
+
+lemma srincr_add tb sz1 sz2 cur at len:
+ 0 <= sz1 => 0 <= sz2 =>
+ srincr (sz1+sz2) cur at len
+ = srincr sz1 cur at len
+   + srincr sz2 (cur+sz1) (srat sz1 cur at len tb) (srlen sz1 cur at len).
+proof. smt(). qed.
+
+lemma srfnsh_add sz1 sz2 cur at len tb:
+ 0 <= sz1 => 0 <= sz2 =>
+ srfnsh (sz1+sz2) cur at len tb
+ = (srfnsh sz1 cur at len tb
+    \/ srfnsh sz2 (cur+sz1) (srat sz1 cur at len tb) (srlen sz1 cur at len) (srtb sz1 cur at len tb)).
+proof. smt(). qed.
+
+lemma srat_add sz1 sz2 cur at len tb:
+ 0 <= sz1 => 0 <= sz2 =>
+ srat (sz1+sz2) cur at len tb
+ = srat sz1 cur at len tb
+   + srincr sz2 (cur+sz1) (srat sz1 cur at len tb) (srlen sz1 cur at len)
+   + b2i (srfnsh sz2 (cur+sz1) (srat sz1 cur at len tb) (srlen sz1 cur at len) (srtb sz1 cur at len tb)).
+proof. smt(). qed.
+
+lemma srlen_add tb sz1 sz2 cur at len:
+ 0 <= sz1 => 0 <= sz2 => 0 <= len =>
+ srlen (sz1+sz2) cur at len
+ = srlen sz2 (cur+sz1) (srat sz1 cur at len tb) (srlen sz1 cur at len).
+proof. smt(). qed.
+
+lemma srtb_add sz1 sz2 cur at len tb:
+ 0 <= sz1 => 0 <= sz2 =>
+ srtb (sz1+sz2) cur at len tb
+ = if srfnsh sz1 cur at len tb
+   then 0
+   else srtb sz2 (cur+sz1) (srat sz1 cur at len tb) (srlen sz1 cur at len) (srtb sz1 cur at len tb).
+proof. smt(). qed.
+
+lemma srl_add tb sz1 sz2 cur at l:
+ 0 <= sz1 => 0 <= sz2 =>
+ srl (sz1+sz2) cur at l
+ = srl sz2 (cur+sz1) (srat sz1 cur at (size l) tb) (srl sz1 cur at l).
+proof. 
+move=> ??.
+by rewrite (srincr_add tb) // addzC -drop_drop; smt(size_drop size_ge0).
+qed.
+
+
+op srpre (cur at:int) (l: bytes) (len tb:int) =
+ 0 <= cur /\ 0 <= at /\ 0 <= tb < 256 /\
+ len = size l /\
+ at + size l + b2i (tb<>0) <= 200 /\
+ (cur <= at \/ l=[] /\ tb=0).
+
+lemma srpre_next sz (cur at:int) (l: bytes) (len tb:int):
+ 0 <= sz =>
+ srpre cur at l len tb =>
+ srpre (cur+sz) (srat sz cur at len tb) (srl sz cur at l) (srlen sz cur at len) (srtb sz cur at len tb).
+proof.
+move => /> Hsz Hcur Hat Htb0 Htb1 H200 [H|] />;
+smt(size_drop size_ge0).
+qed.
+
+op srspec lw (cur at:int) (l:W8.t list) (len tb:int) =
+ srpre cur at l len tb =>
+ srpre (cur+size lw)
+       (srat (size lw) cur at len tb)
+       (srl (size lw) cur at l)
+       (srlen (size lw) cur at len)
+       (srtb (size lw) cur at len tb)
+ /\ u8prefAbsorb lw (at-cur) l tb.
+
+lemma srpreP cur at l len tb:
+ srpre cur at l len tb => cur <= at \/ l=[] /\ tb=0
+by smt().
+
+lemma srspec_cat lw1 lw2 cur at l len tb:
+ srspec lw1 cur at l len tb =>
+ srspec lw2 (cur+size lw1) (srat (size lw1) cur at len tb) (srl (size lw1) cur at l) (srlen (size lw1) cur at len) (srtb (size lw1) cur at len tb) =>
+ srspec (lw1++lw2) cur at l len tb.
+proof.
+have Hsz1:= (size_ge0 lw1).
+have Hsz2:= (size_ge0 lw2).
+have Hszl:= (size_ge0 l).
+case: (srpre cur at l len tb) => Hpre; last smt().
+move=> H1 H2 _; move: (H1 Hpre) => {H1} [Hpre1 /u8prefAbsorbP H1].
+move: (H2 Hpre1) => {H2} [Hpre2 /u8prefAbsorbP H2].
+rewrite !size_cat srat_add 1..2:/# (srl_add tb) 1..2:/# (srlen_add tb) 1..3:/# srtb_add 1..2:/#.
+split; first smt().
+move: Hpre H1 H2 => /> ????? [Hat|[]->->]; last first.
+ move=> /u8prefAbsorbP /u8prefAbsorb0 T1 /u8prefAbsorbP /u8prefAbsorb0; move: T1=> /= -> -> i.
+ by rewrite cat_nseq 1..2:/# nth_u8zeros size_nseq /#.
+move=> H1 H2 i.
+rewrite nth_cat; case: (i<size lw1) => C1.
+ case: (i < 0) => C2; first by rewrite nth_out 1:/# ifF 1:/#.
+ case: (max 0 (at-cur) <= i) => C3 /=.
+  by rewrite nth_rcons size_cat ifT 1:/# H1 ifT 1:/#; smt(nth_out).
+ by rewrite H1 /= ifF 1:/#.
+rewrite H2 size_cat.
+case: (i < size lw1+size lw2) => C2/=; last first.
+ by rewrite ifF /#.
+case: (max 0 (at - cur) <= i) => C3; last by rewrite ifF 1:/#.
+rewrite ifT 1:/# nth_rcons.
+case: (i - max 0 (at - cur) = size l) => C4.
+ rewrite ifT ?size_drop'; smt(nth_out nth_cat).
+move: (srpreP _ _ _ _ _ Hpre1); case:( cur + size lw1 <= srat (size lw1) cur at (size l) tb) => C5/=; last first.
+ by move => [] -> -> /=; smt(nth_out size_cat).
+rewrite size_drop 1:/#.
+case: (i = size lw1) => HHH.
+ rewrite HHH /=.
+ case: (srat (size lw1) cur at (size l) tb = cur + size lw1) => CC; last smt().
+ rewrite CC /= ler_maxl 1:/# /=.
+ case: (size l = srincr (size lw1) cur at (size l)) => CCC.
+  by rewrite CCC /= ifT 1:/#; smt(nth_out nth_cat).
+ by rewrite ifF 1:/# nth_drop; smt(nth_cat).
+rewrite ifF.
+ move: C5; case: (tb=0) => C6; first smt().
+ rewrite /srfnsh C6 size_ge0 /=.
+ case: ((0 <= at - cur < size lw1 && at + size l < cur + size lw1)) => C7/=; last smt().
+ rewrite b2i1 /srincr. 
+ have ?: size l < (cur + size lw1 - at) by smt().
+ rewrite ler_minl 1:/# ifT 1:/# => ?.
+ rewrite (ler_maxr _ (size l)); first smt(size_ge0).
+ have ->: at + size l = cur + size lw1 - 1 by smt().
+ by rewrite /= ler_maxr /#.
+by rewrite nth_drop 1..2:/# /srfnsh /srincr; smt(nth_out nth_cat).
+qed.
+
+lemma srspec_ahead lw cur at l len1 len tb1 tb:
+ size l = len =>
+ 0 <= len1 <= len =>
+ 0 <= tb1 < 256 =>
+ 0 <= at-cur < 8 =>
+ cur + size lw <= at + len1 => 
+ srspec lw cur at (take len1 l) len1 tb1 =>
+ srspec lw cur at l len tb.
+proof.
+move => Elen Elen1 Htb Hat Hlen H Hpre; split.
+ by apply srpre_next; smt(size_ge0).
+move: (H _).
+ split; first smt().
+ split; first smt().
+ split; first smt().
+ split; first smt(size_take).
+ split.
+  rewrite size_take 1:/#. 
+  admit (* remove keccakstate size from srpre!!! *).
+ smt().
+move => [_ HH].
+(* e para que é isto? *)
+admitted.
+
+(*
+move=> Hpre; split; first by rewrite srpre_next.
+move: (H1 _); first smt(size_memread).
+move=> []? E i.
+rewrite E size_to_list !nth_rcons size_memread 1:/#. 
+rewrite ler_maxr 1:/#.
+case: (at - cur <= i < 8) => C //=.
+rewrite size_memread 1:/#.
+smt(nth_memread).
+qed.
+
+Hcur: 0 <= at - cur < 8
+Hlen: 0 <= len <= len2
+Hat: at1 = cur + 8
+H1: srspec (u64bytes w1) cur at (memread m buf len) len 0
+H: at1 = srat (size (u64bytes w1)) cur at len 0 /\
+   buf1 = buf + srincr (size (u64bytes w1)) cur at len /\
+   len1 = srlen (size (u64bytes w1)) cur at len /\
+   0 = srtb (size (u64bytes w1)) cur at len 0
+L: int := len2 - len
+_: at1 = min (cur + 8) (at + len)
+------------------------------------------------------------------------
+srspec (u64bytes w1) cur at (memread m buf (len + L)) (len + L) 0
+*)
+lemma srspec_tb w cur at l len tb:
+ srspec (u64bytes w) cur at l len 0 =>
+ cur <= at =>
+ at + len < cur + 8 =>
+ srspec (u64bytes (w `|` (W64.of_int (tb %% 256) `<<` W8.of_int (8 * (at + len - cur))))) cur at l len tb.
+proof.
+move => H Hcur Hl Hpre; rewrite size_to_list; split; first by rewrite srpre_next.
+have HHpre: srpre cur at l len 0 by smt().
+move: (H HHpre) => {H} [_ H].
+move=> i; rewrite size_to_list nth_rcons u64bytes_or ler_maxr 1:/#.
+case: (at - cur <= i < 8) => C; last first.
+ rewrite H ler_maxr 1:/# size_to_list C /=.
+ case: (i < 0 \/ 8 <= i) => C2.
+  by rewrite nth_out // size_to_list /#.
+ rewrite shl_shlw; first smt(size_ge0).
+ rewrite (nth_u64bytes_shl [W8.of_int tb]).
+   smt(size_ge0).
+  move=> j; case: (j=0) => C4.
+   rewrite size_to_list nth_to_list ifT 1:/# ifT 1:/#.
+   by rewrite of_int_bits8_div 1:/# C4 /= /#.
+  case: (0 <= j < 8) => C5 //.
+   rewrite nth_to_list of_int_bits8_div // divz_small //. 
+    split; first smt().
+    move=> _; rewrite exprM. 
+    apply (ltr_le_trans W8.modulus); first smt().
+    by rewrite {1}(:W8.modulus=W8.modulus^1) 1:/#; smt(ler_eexpr).
+   smt().
+  by rewrite nth_out ?size_to_list // /#.
+ by rewrite ifF; smt(size_ge0).
+case: (i-(at-cur) < size l) => C2.
+ rewrite shl_shlw 1:/# (nth_u64bytes_shl [W8.of_int tb]) 1:/#.
+  move=> j; rewrite ler_maxr // size_to_list.
+  case: (j<0 \/ 8 <= j) => ?.
+   rewrite nth_out.
+    by rewrite size_to_list /#.
+   by rewrite ifF 1:/#.
+  case: (j=0) => C3.
+   rewrite ifT 1:/# C3 /= get_u64bytes /=.
+   by rewrite of_int_bits8_div /#.
+  rewrite /= C3 /= get_u64bytes.
+  rewrite of_int_bits8_div 1:/# divz_small //.
+  split; first smt().
+  move=> _; rewrite exprM.
+  by apply (ltr_le_trans W8.modulus); smt(ler_eexpr).
+ by rewrite H nth_rcons size_to_list ifT 1:/# ifT 1:/# (nth_out _ [W8.of_int tb]) 1:/# orw0 /#.
+rewrite H size_to_list nth_rcons.
+case: (max 0 (at - cur) <= i < 8) => C3; last first.
+ by rewrite or0w shl_shlw 1:/# (nth_u64bytes_shl [W8.of_int tb]) /#.
+rewrite ifF 1:/# or0w shl_shlw. 
+ smt(size_ge0).
+rewrite (nth_u64bytes_shl [W8.of_int tb]); last smt().
+ smt(size_ge0).
+move=> j; case: (j=0) => C4.
+ rewrite size_to_list nth_to_list ifT 1:/# ifT 1:/#.
+ by rewrite of_int_bits8_div 1:/# C4 /= /#.
+rewrite size_to_list ler_maxr 1:/# C4 /=.
+case: (0 <= j < 8) => C5 //.
+ rewrite nth_to_list of_int_bits8_div // divz_small //. 
+ split; first smt().
+ move=> _; rewrite exprM. 
+ apply (ltr_le_trans W8.modulus); first smt().
+ by rewrite {1}(:W8.modulus=W8.modulus^1) 1:/#; smt(ler_eexpr).
+by rewrite nth_out //.
+qed.
+
+lemma srspec_tb_ahead w cur at l len tb:
+ srspec (u64bytes w) cur at l len 0 =>
+ cur + 8 <= at + len =>
+ srspec (u64bytes w) cur at l len tb.
+proof.
+move=> H Hcur.
+admitted.
+
+lemma srspec_u64 w cur at l len :
+ 0 <= at-cur < 8 =>
+ u8prefAt (u64bytes w) 0 l =>
+ srspec (u64bytes (w `<<<` 8*(at-cur))) cur at l len 0.
+proof.
+move=> Hcur Hw Hpre.
+split.
+ by rewrite size_to_list srpre_next.
+move=> i; rewrite size_to_list.
+case: (0 <= i < 8) => Hi; last first.
+ by rewrite nth_out ?size_to_list /#.
+rewrite ler_maxr 1:/# (nth_u64bytes_shl l) 1:/# //.
+smt(nth_rcons nth_out).
+qed.
+
+lemma srspec_u32 n w cur at l:
+ 0 <= at-cur < 8 =>
+ n = min (cur + 8 - at) 4 =>
+ 4 <= size l =>
+ srspec (u64bytes (w `<<<` 8*(at-cur))) cur at (take 4 l)  4 0.
+proof.
+move=> Hcur Hw Hpre.
+admitted(*
+split.
+ by rewrite size_to_list srpre_next.
+move=> i; rewrite size_to_list.
+case: (0 <= i < 8) => Hi; last first.
+ by rewrite nth_out ?size_to_list /#.
+rewrite ler_maxr 1:/#.
+case: (at-cur <= i < 8) => C.
+ by rewrite ifF 1:/# (nth_u64bytes_shl l) // ifT /#.
+by rewrite  (nth_u64bytes_shl l) // ifF /#.
+qed.*).
+
+lemma srspec_shl w cur at l len:
+ 0 <= at-cur < 8 =>
+ u8prefAt (u64bytes w) 0 l =>
+ srspec (u64bytes (w `<<<` 8*(at-cur))) cur at l len 0.
+proof.
+move=> Hcur Hw Hpre.
+split.
+ by rewrite size_to_list srpre_next.
+move=> i; rewrite size_to_list.
+admitted(*
+ by rewrite nth_out ?size_to_list /#.
+rewrite ler_maxr 1:/#.
+case: (at-cur <= i < 8) => C.
+ by rewrite ifF 1:/# (nth_u64bytes_shl l) // ifT /#.
+by rewrite  (nth_u64bytes_shl l) // ifF /#.
+qed.*).
+
+lemma srspec_split l1 l2 w1 w2 cur at l len at1:
+ 0 <= at-cur < 8 =>
+ l = l1++l2 =>
+ at1 = at + size l1 =>
+ at1 < cur + 8 =>
+ u8prefAt (u64bytes w2) 0 l2 =>
+ srspec (u64bytes w1) cur at l1 (len - size l2) 0 =>
+ srspec (u64bytes (w1 `|` (w2 `<<<` 8*(at1-cur)))) cur at l len 0.
+proof.
+move=> Hcur -> -> Hat Hw2 H1 Hpre; split.
+ by rewrite size_to_list; apply srpre_next.
+move: (H1 _); first smt(size_ge0 size_cat).
+move=> {H1} []_ Hw1 i.
+rewrite size_to_list u64bytes_or Hw1 ler_maxr 1:/# size_to_list (nth_u64bytes_shl l2) //.
+ smt(size_ge0).
+case: (at - cur <= i < 8) => C1; last first.
+ rewrite or0w; smt(nth_out size_ge0).
+rewrite !nth_rcons nth_cat ?size_cat.
+case: (i - (at - cur) = size l1) => C2.
+ rewrite ifF 1:/# or0w; smt(nth_out).
+case: (at + size l1 - cur <= i < 8) => C3.
+ rewrite nth_out 1:/# or0w.
+ smt(nth_out size_ge0).
+smt(nth_out size_ge0).
+qed.
+
+lemma srspec_w4_w2 w1 w2 cur at at1 l len:
+ 0 <= size l < 8 =>
+ srspec (u64bytes w1) cur at (take (size l%/4*4) l) len 0 =>
+ at1 = srat 8 cur at len 0 =>
+ srspec (u64bytes (w1 `|` w2 `<<<` 8*(at1-cur))) cur at (take (size l%/2*2) l) (size l%/2*2) 0.
+admitted.
+
+lemma srspec_w2_w1 w1 w2 cur at at1 l len:
+ 0 <= size l < 8 =>
+ srspec (u64bytes w1) cur at (take (size l%/2*2) l) (size l%/2*2) 0 =>
+ at1 = srat 8 cur at len 0 =>
+ srspec (u64bytes (w1 `|` w2 `<<<` 8*(at1-cur))) cur at l len 0.
+admitted.
+
+
+(***************************************
+      MEMORY reads/writes
+****************************************)
+
+
+
+lemma drop_srl_memread (mem: global_mem_t) off len sz cur at:
+ 0 <= sz =>
+ drop (srincr sz cur at len) (memread mem off len)
+ = memread mem (off+srincr sz cur at len) (len-srincr sz cur at len).
+proof.
+move=> Hsz; apply (eq_from_nth W8.zero).
+rewrite size_drop' /srincr !size_memread' 1:/#.
+rewrite size_drop' size_memread' => i Hi.
+rewrite nth_memread /srl' 1:/# nth_drop; 1..2: smt(size_ge0).
+by rewrite nth_memread; smt(size_ge0).
+qed.
+
+op msubreadpre m (lw: W8.t list) (cur at off len tb:int) =
+ srpre cur at (memread m off len) len tb.
+
+op msubread (m : global_mem_t) lw (cur at off len tb:int) at2 off2 len2 tb2 =
+ srspec lw cur at (memread m off len) len tb
+ /\ at2 = srat (size lw) cur at len tb
+ /\ off2 = off + srincr (size lw) cur at len
+ /\ len2 = len - srincr (size lw) cur at len
+ /\ tb2 = srtb (size lw) cur at len tb.
+
+lemma msubread_nil (m: global_mem_t) (cur at off len tb: int):
+ msubread m [] cur at off len tb at off len tb
+by smt().
+
+lemma msubread0 (m: global_mem_t) (lw:W8.t list) (cur at off len tb: int):
+ lw=u8zeros (size lw) => (len < 0 \/ at<cur \/ cur+size lw <= at \/ len=0 /\ tb=0) => msubread m lw cur at off len tb at off len tb.
+proof.
+move=> -> [H|[H|[|[->->]]]]; rewrite /msubread size_nseq.
++ split; last smt().
+  by apply absurd => _; rewrite /srpre size_memread' /#.
++ split; last smt().
+  by move=> Hpre; rewrite size_nseq; smt(nth_u8zeros).
++ rewrite ler_maxr; first smt(size_ge0).
+  move=> H; split; last smt().
+  move=> Hpre; split.
+   by rewrite srpre_next; smt(size_ge0).
+  rewrite u8prefAbsorbP => i; rewrite size_nseq size_memread' nth_u8zeros.
+  case: (0 <= i < size lw) => C; last smt().
+  by rewrite nth_out /#.
+split; last smt().
+by move=> ?; rewrite memread0 size_nseq; smt(size_ge0 nth_u8zeros).
+qed.
+
+lemma msubread_cat m lw1 lw2 (cur at dlt len tb:int) at1 dlt1 len1 tb1 at2 dlt2 len2 tb2:
+ msubread m lw1 cur at dlt len tb at1 dlt1 len1 tb1 =>
+ msubread m lw2 (cur+size lw1) at1 dlt1 len1 tb1 at2 dlt2 len2 tb2 =>
+ msubread m (lw1++lw2) cur at dlt len tb at2 dlt2 len2 tb2.
+proof.
+rewrite /msubread => /= [#]H1 Hat1 Hdlt1 Hlen1 Htb1.
+move => /= [#]H2 Hat2 Hdlt2 Hlen2 Htb2.
+split; last first.
+ by rewrite size_cat srat_add; smt(size_ge0).
+move => Hpre; move:(Hpre).
+have Hl: memread m dlt1 len1 = srl (size lw1) cur at (memread m dlt len)
+ by smt(size_ge0 drop_srl_memread).
+by apply (srspec_cat lw1 lw2 cur at (memread m dlt len) len tb) => // /#.
+qed.
+
+
+
+lemma msubread_u64 m _cur _at _buf _len:
+ 8 <= _len =>
+ 0 <= _at-_cur < 8 =>
+ msubread m (u64bytes (loadW64 m _buf `<<<` 8 * (_at - _cur))) _cur _at
+            _buf _len 0 (_cur + 8) (_buf + (_cur + 8 - _at)) (_len - (_cur + 8 - _at)) 0.
+proof.
+move=> Hlen Hat; rewrite /msubread; split; last first.
+ by rewrite size_to_list; smt(size_memread).
+apply srspec_shl=>  //.
+ admit.
+qed.
+
+
+lemma msubread_ahead m w1 cur at buf len at1 buf1 len1 len2:
+ 0 <= at-cur < 8 =>
+ 0 <= len <= len2  =>
+ at1 = cur+8 =>
+ msubread m (u64bytes w1) cur at buf len 0
+          at1 buf1 len1 0 =>
+ msubread m (u64bytes w1) cur at buf len2 0
+          at1 buf1 (len2-(cur+8-at)) 0.
+proof.
+move=> Hcur Hlen Hat [H1 H].
+pose L:= len2-len.
+have {1}->: len2 = len + L by smt().
+have ?: at1 = min (cur+8) (at+len). 
+ by move: H Hat => />; rewrite /srfnsh /srincr size_to_list !ifT 1..2:/# b2i0 /= => _ /#.
+split; last first.
+ by rewrite /srfnsh /srincr size_to_list /#.
+move=> Hpre; split; first by rewrite srpre_next.
+move: (H1 _); first smt(size_memread).
+move=> []? E i.
+rewrite E size_to_list !nth_rcons size_memread 1:/#. 
+rewrite ler_maxr 1:/#.
+case: (at - cur <= i < 8) => C //=.
+rewrite size_memread 1:/#.
+smt(nth_memread).
+qed.
+
+lemma msubread_w4_u2 m w1 cur at buf len at1 buf1 len1 dlt:
+ 0 <= at-cur < 8 =>
+ 0 <= len < 8 =>
+ at1 < cur+8 =>
+ 2 <= len%%4 =>
+ at + dlt = min (cur+8) (at+len%/4*4+2) =>
+ msubread m (u64bytes w1) cur at buf (len%/4*4) 0
+          at1 buf1 len1 0 =>
+ msubread m
+    (u64bytes (w1 `|` (zeroextu64 (loadW16 m buf1) `<<<` 8*(at1-cur))))
+    cur at buf (len%/2*2) 0
+    (at+dlt) (buf+dlt) (len%/2*2-dlt) 0.
+proof.
+move=> Hcur Hlen Hat Hl Hdlt [Hspec1 H]; split; last first.
+ by rewrite /srfnsh /srincr size_to_list /= /#.
+have ?: at1 = at + len%/4*4.
+ by move: H Hat => />; rewrite /srfnsh /srincr size_to_list !ifT 1..2:/# b2i0 /= /#.
+move: H => />.
+pose AT1 := srat (size (u64bytes w1)) cur at (len %/ 4 * 4) 0.
+pose W2 := zeroextu64 (loadW16 _ _).
+apply (srspec_split (memread m buf (len%/4*4)) (memread m (buf+len%/4*4) (len%%4%/2*2)) w1 W2 cur at (memread m buf (len%/2*2)) (len%/2*2) AT1) => //.
++ by rewrite -memread_add /#.
++ by rewrite size_memread 1:/# /AT1 size_to_list /srfnsh /srincr !ifT 1..2:/# /= b2i0 /#.
++ admit (*
+  u8window (u64bytes W2) 0 (memread m (buf + len %/ 4 * 4) (len %% 4 %/ 2 * 2)) 0
+*).
+by rewrite size_memread /#.
+qed.
+
+
+
+
+op msubwrite (m m2: global_mem_t) lw (buf len:int) buf2 len2 =
+ m2 = stores m buf (take len lw)
+ /\ buf2 = buf + min (size lw) (max 0 len)
+ /\ len2 = len - min (size lw) (max 0 len).
+
+
+lemma msubwrite_cat m m1 m2 lw1 lw2 buf len buf1 len1 buf2 len2:
+ msubwrite m m1 lw1 buf len buf1 len1 =>
+ msubwrite m1 m2 lw2 buf1 len1 buf2 len2 =>
+ msubwrite m m2 (lw1++lw2) buf len buf2 len2.
+proof.
+move=> />; split; last smt(size_ge0 size_cat).
+rewrite take_cat; case: (len < size lw1) => C.
+ by rewrite (take_le0 (len -_)) 1:/# store0.
+rewrite stores_cat; congr.
+  by rewrite take_oversize 1:/#.
+ smt(size_ge0).
+congr; smt(size_ge0).
+qed.
+
+
+
+(* lossless assertions *)
+
 lemma m_ilen_read_upto8_at_ll: islossless M.__m_ilen_read_upto8_at
 by islossless.
 
@@ -258,7 +859,7 @@ by islossless.
 lemma m_ilen_write_upto8_ll: islossless M.__m_ilen_write_upto8
 by islossless.
 
-lemma m_ilen_write_upto16_ll: islossless M.__m_ilen_write_upto8
+lemma m_ilen_write_upto16_ll: islossless M.__m_ilen_write_upto16
 by islossless.
 
 lemma m_ilen_write_upto32_ll: islossless M.__m_ilen_write_upto32
@@ -269,6 +870,403 @@ by islossless.
 
 lemma m_rlen_write_upto8_ll: islossless M.__m_rlen_write_upto8
 by islossless.
+
+
+(*
+lemma subread_w8_trail buf off cur dlt len trail at dlt1 len1 at1 w:
+ trail <> 0 =>
+ 0 <= len < 8 =>
+ 0 <= at-cur < 8 =>
+ at1 < cur+8 =>
+ subread_spec 8 buf off dlt len 0 cur at dlt1 len1 0 at1 (u64bytes w) =>
+ subread_spec 8 buf off dlt len trail cur at dlt1 len1 0 (at1+1)
+   (u64bytes
+     (w `|` (W64.of_int (trail %% 256) `<<` W8.of_int (8 * (at1 - cur))))).
+proof.
+
+
+lemma subread_w4_u16 n1 buf off cur dlt len at dlt1 len1 at1 w:
+ 0 <= len < 8 =>
+ 2 <= len%%4 =>
+ 0 <= at-cur < 8 =>
+ at+n1 = min (cur+8) (at+len%/4*4+2) =>
+ subread_spec 8 buf off dlt (len%/4*4) 0 cur at
+   dlt1 len1 0 at1 (u64bytes w) =>
+ subread_spec 8 buf off dlt (len%/2*2) 0 cur at
+   (dlt+n1) (len%/2*2-n1) 0 (at+n1)
+   (u64bytes
+     (w `|`
+      (zeroextu64
+         (get16_direct (WA.init8 ("_.[_]" buf)) (off + dlt1)) `<<<` 8*(at1-cur)))).
+proof.
+move=> Hlen Hlen2 Hcur Hat H _ Hpre; split; first smt().
+have Hpre': subread_pre cur at off dlt (len %/ 4 * 4) 0 by smt().
+split.
+ apply (eq_from_nth W8.zero).
+  rewrite size_to_list size_take // size_cat size_nseq ler_maxr //=.
+  by rewrite size_drop 1:/# !size_cat size_sub 1:/# size_nseq /= /#.
+ move=> i; rewrite size_to_list => Hi.
+ rewrite get_u64bytes orb8E bits8_u64_shl8 //.
+ rewrite (u64bits8_subread _ _ _ _ _ _ _ _ _ _ _ _ _ Hpre' H).
+ rewrite bits8_zeroextu64_16 !nth_bytes_at // get16_bytes 1..2:/#.
+ case: (0 <= at - cur <= i < 8) => ?.
+  case: (i < at1 - cur) => ?.
+   by rewrite orw0 !nth_cat !size_sub 1..2:/# /= !ifT 1..2:/# !nth_sub /#.
+  case: (0 <= i - (at1 - cur) < 2) => ?.
+   rewrite nth_sub 1:/# !nth_cat !size_sub 1..2:/# ifF 1:/# ifT 1:/# /=.
+   by rewrite nth_sub /#.
+  by rewrite orw0 !nth_cat !size_sub 1..2:/# ifF 1:/# ifF 1:/#.
+ rewrite or0w; case: (i < at1-cur) => ? //.
+ case: (0 <= i - (at1 - cur) < 2) => ? //.
+ by rewrite nth_sub /#.
+smt().
+qed.
+
+lemma subread_w4_ahead buf off cur dlt len at dlt1 len1 at1 w:
+ 0 <= len < 8 =>
+ 0 <= at-cur < 8 =>
+ at1 = cur+8 =>
+ subread_spec 8 buf off dlt (len%/4*4) 0 cur at
+   dlt1 len1 0 at1 (u64bytes w) =>
+ subread_spec 8 buf off dlt (len%/2*2) 0 cur at
+   dlt1 (len%/2*2-(cur+8-at)) 0 at1 (u64bytes w).
+proof.
+move=> Hlen Hcur Hat H _ Hpre; split; first smt().
+split.
+ move: (H _ _); 1..2:smt().
+ move => |> _ -> ??.
+ apply (eq_from_nth W8.zero); rewrite !size_bytes_at // => k Hk.
+ rewrite !nth_bytes_at //; first smt().
+ case: (0 <= at - cur <= k < 8) => ?//.
+ rewrite !nth_cat !size_sub 1..2:/#.
+ case: (cur + k - at < len %/ 4 * 4) => ?.
+  by rewrite ifT 1:/# !nth_sub /#.
+ by rewrite ifF 1:/#.
+smt().
+qed.
+*)
+
+(*
+  admit (* by apply (subread_u32 (min (_cur+8-_at) 4) _buf _off _dlt _cur _at _ _); smt().
+_: _cur <= _at
+_: _at < _cur + 8
+_: _len < 8
+_: _len <> 0 \/ _tb <> 0
+_: 4 <= _len
+_: 0 <= _at - _cur
+_: _at - _cur < 8
+------------------------------------------------------------------------
+msubread Glob.mem{`&hr}
+  (u64bytes (zeroextu64 (loadW32 Glob.mem{`&hr} _buf) `<<<` 8 * (_at - _cur)))
+  _cur _at _buf 4 0 (_at + min (_cur + 8 - _at) 4)
+  (_buf + min (_cur + 8 - _at) 4) (4 - min (_cur + 8 - _at) 4) 0
+*).
+
+lemma msubread_u64 m _cur _at _buf _len _tb:
+ 8 <= _len =>
+ 0 <= _at-_cur < 8 =>
+ msubread m (u64bytes (loadW64 m _buf `<<<` 8 * (_at - _cur))) _cur _at
+            _buf _len _tb (_cur + 8) (_buf + (_cur + 8 - _at)) (_len - (_cur + 8 - _at)) _tb.
+proof.
+move=> Hlen Hat; rewrite /msubread; split.
+ apply srspec_u64; first smt().
+ admit.
+by rewrite size_to_list; smt(size_memread).
+qed.
+*)
+
+(*
+lemma subread_u32 n _buf _off _dlt _cur _at :
+ 0 <= _at-_cur < 8 =>
+ n = min (_cur + 8 - _at) 4 =>
+ subread_spec 8 _buf _off _dlt 4 0 _cur
+   _at (_dlt+n) (4-n) 0 (_at+n)
+   (u64bytes (zeroextu64 (get32_direct (WA.init8 ("_.[_]" _buf)) (_off + _dlt)) `<<<`
+      8 * (_at - _cur))).
+proof.
+move=> Hen Hcur _ Hpre; split; first smt().
+split; last smt().
+apply (eq_from_nth W8.zero).
+ rewrite size_to_list size_take // size_cat size_nseq ler_maxr //=.
+ by rewrite size_drop 1:/# !size_cat size_sub 1:/# size_nseq /= /#.
+move=> i; rewrite size_to_list => Hi.
+rewrite nth_bytes_at //.
+rewrite get_u64bytes bits8_u64_shl8 //.
+case: (_at-_cur <= i) => C //=.
+ rewrite ifF 1:/# ifT 1:/# nth_cat size_sub 1:/# bits8_zeroextu64_32.
+ rewrite (:i - (_at - _cur)=_cur + i - _at) 1:/#; case: (0<= _cur + i - _at < 4) => ? //.
+  by rewrite get32_bytes /#.
+ case: (_cur + i - _at < 4) => // ?.
+ by rewrite nth_sub /#.
+by rewrite ifT 1:/#.
+qed.
+*)
+
+
+
+
+lemma m_ilen_read_upto8_at_h _buf _len _tb _cur _at:
+ hoare [
+ M.__m_ilen_read_upto8_at
+ : buf=_buf /\ lEN=_len /\ tRAIL=_tb /\ cUR=_cur /\ aT=_at
+ ==> msubread Glob.mem (u64bytes res.`5) _cur _at _buf _len _tb
+              res.`4 res.`1 res.`2 res.`3
+ ]. 
+proof.
+proc; simplify.
+if => //.
+ by auto => |> &m [[H|H]|H]; apply msubread0; rewrite size_to_list ?u64bytes0 // /#.
+sp; if => //.
+ (* 8 <= lEN *)
+ wp; ecall (SHLQ_h w (aT-cUR)); auto => |> *.
+ split; first smt().
+ move=> ??.
+ admit (* by apply msubread_u64.*).
+conseq (: _cur <= _at < _cur+8 /\ 0 <= _len < 8 /\ (_len<>0 \/ _tb<>0) 
+         /\ buf=_buf /\ cUR=_cur /\ tRAIL=_tb
+         /\ lEN=_len /\ aT=_at==> _).
+ by move => /> /#.
+pose n0 := min (_cur + 8 - _at) (_len %/ 4 * 4).
+seq 1: ( #[:2,3,5:6]pre
+       /\ msubread Glob.mem (u64bytes w) _cur _at _buf (_len %/ 4 * 4) 0 aT buf (_len %/ 4 * 4-n0) 0
+       /\ buf = _buf+n0 /\ lEN = _len - n0 /\ aT=_at+n0).
+ if => //.
+  (* 4 <= lEN  *)
+  wp; ecall (SHLQ_h w (aT-cUR)); auto => |> *.
+  split; first smt().
+  move=> ??.
+  rewrite /n0.
+  have ->: _len %/ 4 * 4 = 4 by smt().
+  have ->: (_buf + if _cur + 8 <= _at + 4 then _cur + 8 - _at else 4)
+          = _buf + min (_cur+8-_at) 4 by smt().
+  have ->: (if _cur + 8 <= _at + 4 then _cur + 8 else _at + 4)
+          = _at + min (_cur+8-_at) 4 by smt().
+  split; last smt().
+  admit (* by apply (subread_u32 (min (_cur+8-_at) 4) _buf _off _dlt _cur _at _ _); smt().
+_: _cur <= _at
+_: _at < _cur + 8
+_: _len < 8
+_: _len <> 0 \/ _tb <> 0
+_: 4 <= _len
+_: 0 <= _at - _cur
+_: _at - _cur < 8
+------------------------------------------------------------------------
+msubread Glob.mem{`&hr}
+  (u64bytes (zeroextu64 (loadW32 Glob.mem{`&hr} _buf) `<<<` 8 * (_at - _cur)))
+  _cur _at _buf 4 0 (_at + min (_cur + 8 - _at) 4)
+  (_buf + min (_cur + 8 - _at) 4) (4 - min (_cur + 8 - _at) 4) 0
+*).
+ auto => |> ???????; split; last smt().
+ rewrite /n0.
+ have ->: (_len %/ 4 * 4 - min (_cur + 8 - _at) (_len %/ 4 * 4)) = _len %/ 4 * 4 by smt().
+ by apply msubread0; rewrite u64bytes0 size_nseq /#.
+pose n1 := min (_cur+8-_at) (_len %/ 2 * 2).
+exlim aT => at1; exlim lEN => len1; exlim buf => buf1.
+conseq (: _cur <= _at < _cur+8 /\ 0 <= _len < 8 /\ (_len<>0 \/ _tb<>0) 
+         /\ cUR=_cur /\ tRAIL=_tb /\ buf=buf1 /\ lEN=len1 /\ aT=at1
+         /\ msubread Glob.mem (u64bytes w) _cur _at _buf (_len%/4*4) 0
+                     at1 buf1 (_len %/ 4 * 4 - n0) 0
+         /\ buf1=_buf+n0 /\ len1=_len-n0 /\ at1=_at+n0
+         ==> _).
+ by move => />.
+seq 1: ( #[/:7]pre
+      /\ msubread Glob.mem (u64bytes w) _cur _at _buf (_len %/ 2 * 2) 0
+                  aT buf (_len%/2*2-n1) 0
+      /\ buf=_buf+n1 /\ lEN=_len-n1 /\ aT=_at+n1).
+ if => //.
+  (* 2 <= lEN *)
+  wp; ecall (SHLQ_h t16 (aT-cUR)); auto => |> ?????? H1??.
+  split; first smt().
+  move=> ??; split; last smt().
+  rewrite -!addzA.
+  have ->: (n0 + if _cur + 8 <= _at + (n0 + 2) then _cur + (8 - (_at + n0)) else 2)=n1 by smt().
+  have ->: (if _cur + 8 <= _at + (n0 + 2) then _cur + 8 else _at + (n0 + 2))=_at+n1 by smt().
+  rewrite (addzA _at).
+admit(*   by apply (subread_w4_u16 n1 _buf _off _ _ _ _ _ _ _ _ _ _ _ _ H1); smt().
+msubread Glob.mem{`&hr}
+  (u64bytes
+     (w{`&hr} `|`
+      (zeroextu64 (loadW16 Glob.mem{`&hr} (_buf + n0)) `<<<`
+       8 * (_at + n0 - _cur)))) _cur _at _buf (_len %/ 2 * 2) 0 (_at + n1)
+  (_buf + n1) (_len %/ 2 * 2 - n1) 0
+*).
+ auto => |> &m ?????H.
+ rewrite negb_and; move => [?|?]; last smt().
+ have En0: n0 = _cur+8-_at by smt().
+ have En1: n1 = n0 by smt().
+ split; last smt().
+ rewrite En1 {2}En0.
+admit (*  by apply (subread_w4_ahead _buf _off _ _ _ _ _ _ _ _ _ _ _ H); smt().*).
+pose n2 := min (_cur+8-_at) _len.
+exlim aT => at2; exlim lEN => len2; exlim buf => buf2.
+conseq (: _cur <= _at < _cur+8 /\ 0 <= _len < 8 /\ (_len<>0 \/ _tb<>0) 
+         /\ cUR=_cur /\ tRAIL=_tb /\ buf=buf2 /\ lEN=len2 /\ aT=at2
+         /\ msubread Glob.mem (u64bytes w) _cur _at _buf (_len%/2*2) 0
+                     at2 buf2 (_len%/2*2 - n1) 0
+         /\ buf2=_buf+n1 /\ len2=_len-n1 /\ at2=_at+n1
+         ==> _).
+ by move => />.
+seq 1: ( #[/:7]pre
+       /\ msubread Glob.mem (u64bytes w) _cur _at _buf _len 0
+                   aT buf (_len-n2) 0
+       /\ buf=_buf+n2 /\ lEN=_len-n2 /\ aT=_at+n2).
+ if => //.
+  (* 1 <= lEN *)
+  wp; ecall (SHLQ_h t8 (aT-cUR)); auto => |> ?????? H1??.
+  split; first smt(). 
+  move=> ??; split; last smt().
+  rewrite -!addzA.
+  have ->: n1+1=n2 by smt().
+  rewrite (addzA _at).
+  admit (*by apply (subread_w2_u8 n2 _buf _off _ _ _ _ _ _ _ _ _ _ _ _ H1); smt().
+msubread Glob.mem{`&hr}
+  (u64bytes
+     (w{`&hr} `|`
+      (zeroextu64 (loadW8 Glob.mem{`&hr} (_buf + n1)) `<<<`
+       8 * (_at + n1 - _cur)))) _cur _at _buf _len 0 (_at + n1 + 1)
+  (_buf + n1 + 1) (_len - n2) 0
+*).
+ auto => |> &m ?????H.
+ rewrite negb_and; move => [?|?]; last smt().
+ have En1: n1 = _cur+8-_at by smt().
+ have En2: n2 = n1 by smt().
+ split; last smt().
+ rewrite En2 {2}En1.
+ admit(* by apply (subread_w2_ahead _buf _off _ _ _ _ _ _ _ _ _ _ _ H); smt().
+H: msubread Glob.mem{m} (u64bytes w{m}) _cur _at _buf (_len %/ 2 * 2) 0
+     (_at + n1) (_buf + n1) (_len %/ 2 * 2 - n1) 0
+_: ! _at + n1 < _cur + 8
+En1: n1 = _cur + 8 - _at
+En2: n2 = n1
+------------------------------------------------------------------------
+msubread Glob.mem{m} (u64bytes w{m}) _cur _at _buf _len 0 (_at + n1)
+  (_buf + (_cur + 8 - _at)) (_len - n1) 0
+*).
+if => //.
+ auto => |> &m ?????H??.
+ admit (*by apply subread_w8_trail => /#.
+H: msubread Glob.mem{m} (u64bytes w{m}) _cur _at _buf _len 0 (_at + n2)
+     (_buf + n2) (_len - n2) 0
+_: _at + n2 < _cur + 8
+_: _tb <> 0
+------------------------------------------------------------------------
+msubread Glob.mem{m}
+  (u64bytes
+     (w{m} `|` (of_int (_tb %% 256) `<<` of_int (8 * (_at + n2 - _cur)))))
+  _cur _at _buf _len _tb (_at + n2 + 1) (_buf + n2) (_len - n2) 0
+*).
+auto => |> &m ?????H; rewrite negb_and => [[C|C]]; last smt().
+admit (*by apply subread_w8_trail_ahead => /#.
+H: msubread Glob.mem{m} (u64bytes w{m}) _cur _at _buf _len 0 (_at + n2)
+     (_buf + n2) (_len - n2) 0
+C: ! _at + n2 < _cur + 8
+------------------------------------------------------------------------
+msubread Glob.mem{m} (u64bytes w{m}) _cur _at _buf _len _tb (_at + n2)
+  (_buf + n2) (_len - n2) _tb
+*).
+qed.
+
+lemma m_ilen_read_upto8_at_ph _buf _len _tb _cur _at:
+ phoare [
+ M.__m_ilen_read_upto8_at
+ : buf=_buf /\ lEN=_len /\ tRAIL=_tb /\ cUR=_cur /\ aT=_at
+ ==> msubread Glob.mem (u64bytes res.`5) _cur _at _buf _len _tb
+              res.`4 res.`1 res.`2 res.`3
+ ] = 1%r. 
+proof.
+by conseq m_ilen_read_upto8_at_ll (m_ilen_read_upto8_at_h _buf _len _tb _cur _at).
+qed.
+
+lemma m_ilen_read_upto16_at_h _buf _len _tb _cur _at:
+ hoare [
+ M.__m_ilen_read_upto16_at
+ : buf=_buf /\ lEN=_len /\ tRAIL=_tb /\ cUR=_cur /\ aT=_at
+   /\ 0 <= _len
+ ==> msubread Glob.mem (u128bytes res.`5) _cur _at _buf _len _tb
+              res.`4 res.`1 res.`2 res.`3
+ ].
+admitted.
+
+lemma m_ilen_read_upto16_at_ph _buf _len _tb _cur _at:
+ phoare [
+ M.__m_ilen_read_upto16_at
+ : buf=_buf /\ lEN=_len /\ tRAIL=_tb /\ cUR=_cur /\ aT=_at
+   /\ 0 <= _len
+ ==> msubread Glob.mem (u128bytes res.`5) _cur _at _buf _len _tb
+              res.`4 res.`1 res.`2 res.`3
+ ] = 1%r.
+proof.
+by conseq m_ilen_read_upto16_at_ll (m_ilen_read_upto16_at_h  _buf _len _tb _cur _at).
+qed.
+
+lemma m_ilen_read_upto32_at_h _buf _len _tb _cur _at:
+ hoare [
+ M.__m_ilen_read_upto32_at
+ : buf=_buf /\ lEN=_len /\ tRAIL=_tb /\ cUR=_cur /\ aT=_at
+   /\ 0 <= _len
+ ==> msubread Glob.mem (u256bytes res.`5) _cur _at _buf _len _tb
+              res.`4 res.`1 res.`2 res.`3
+ ]. 
+admitted.
+
+lemma m_ilen_read_upto32_at_ph _buf _len _tb _cur _at:
+ phoare [
+ M.__m_ilen_read_upto32_at
+ : buf=_buf /\ lEN=_len /\ tRAIL=_tb /\ cUR=_cur /\ aT=_at
+   /\ 0 <= _len
+ ==> msubread Glob.mem (u256bytes res.`5) _cur _at _buf _len _tb
+              res.`4 res.`1 res.`2 res.`3
+ ] = 1%r. 
+proof.
+by conseq m_ilen_read_upto32_at_ll (m_ilen_read_upto32_at_h  _buf _len _tb _cur _at).
+qed.
+
+
+
+hoare m_ilen_write_upto8_h (_m: global_mem_t) _buf _len _w:
+ M.__m_ilen_write_upto8
+ : buf=_buf /\ lEN=_len /\ w = _w
+ ==> msubwrite _m Glob.mem (u64bytes _w) _buf _len res.`1 res.`2.
+proof.
+proc => /=.
+admitted.
+
+phoare m_ilen_write_upto8_ph (_m: global_mem_t) _buf _len _w:
+ [ M.__m_ilen_write_upto8
+ : buf=_buf /\ lEN=_len /\ w = _w
+ ==> msubwrite _m Glob.mem (u64bytes _w) _buf _len res.`1 res.`2
+ ] = 1%r.
+proof. by conseq m_ilen_write_upto8_ll (m_ilen_write_upto8_h _m _buf _len _w). qed.
+
+hoare m_ilen_write_upto16_h (_m: global_mem_t) _buf _len _w:
+ M.__m_ilen_write_upto16
+ : buf=_buf /\ lEN=_len /\ w = _w
+ ==> msubwrite _m Glob.mem (u128bytes _w) _buf _len res.`1 res.`2.
+proof.
+proc => /=.
+admitted.
+
+phoare m_ilen_write_upto16_ph (_m: global_mem_t) _buf _len _w:
+ [ M.__m_ilen_write_upto16
+ : buf=_buf /\ lEN=_len /\ w = _w
+ ==> msubwrite _m Glob.mem (u128bytes _w) _buf _len res.`1 res.`2
+ ] = 1%r.
+proof. by conseq m_ilen_write_upto16_ll (m_ilen_write_upto16_h _m _buf _len _w). qed.
+
+hoare m_ilen_write_upto32_h (_m: global_mem_t) _buf _len _w:
+ M.__m_ilen_write_upto32
+ : buf=_buf /\ lEN=_len /\ w = _w
+ ==> msubwrite _m Glob.mem (u256bytes _w) _buf _len res.`1 res.`2.
+proof.
+proc => /=.
+admitted.
+
+phoare m_ilen_write_upto32_ph (_m: global_mem_t) _buf _len _w:
+ [ M.__m_ilen_write_upto32
+ : buf=_buf /\ lEN=_len /\ w = _w
+ ==> msubwrite _m Glob.mem (u256bytes _w) _buf _len res.`1 res.`2
+ ] = 1%r.
+proof. by conseq m_ilen_write_upto32_ll (m_ilen_write_upto32_h _m _buf _len _w). qed.
 
 
 
@@ -286,6 +1284,104 @@ clone import PolyArray as A
 clone import WArray as WA
  with op size <- _ASIZE.
 
+(* Some auxiliary lemmata *)
+
+lemma sub0 (buf: W8.t A.t) off:
+ sub buf off 0 = [].
+proof. by rewrite -size_eq0 size_sub /#. qed.
+
+
+lemma size_sub' ['a] (buf:'a A.t) k len:
+ size (sub buf k len) = max 0 len.
+proof.
+case: (0<=len) => H.
+ by rewrite size_sub /#.
+by rewrite /sub mkseq0_le /#.
+qed.
+
+lemma drop_sub (buf: W8.t A.t) off len sz cur at:
+ 0 <= sz =>
+ drop (srincr sz cur at len) (sub buf off len)
+ = sub buf (off+srincr sz cur at len) (len-srincr sz cur at len).
+proof.
+move=> Hsz; apply (eq_from_nth W8.zero).
+rewrite size_drop' /srincr !size_sub' 1:/#.
+rewrite size_drop' size_sub' => i Hi.
+rewrite nth_sub /srl' 1:/# nth_drop; 1..2: smt(size_ge0).
+by rewrite nth_sub; smt(size_ge0).
+qed.
+
+(* The instantiation of the subread spec for arrays *)
+
+op asubread (buf:W8.t A.t) off lw (cur at dlt len tb at2 dlt2 len2 tb2: int) =
+ srspec lw cur at (sub buf (off+dlt) len) len tb
+ /\ at2 = srat (size lw) cur at len tb
+ /\ dlt2 = dlt + srincr (size lw) cur at len
+ /\ len2 = len - srincr (size lw) cur at len
+ /\ tb2 = srtb (size lw) cur at len tb.
+
+lemma asubread0 (buf:W8.t A.t) off lw (cur at dlt len tb:int):
+ lw = u8zeros (size lw) =>
+ len < 0 \/ at < cur \/ cur + size lw <= at \/ len = 0 /\ tb = 0 =>
+ asubread buf off lw cur at dlt len tb at dlt len tb.
+proof.
+move=> -> [H|[H|[|[->->]]]]; rewrite /asubread size_nseq.
++ split; last smt().
+  by apply absurd => _; rewrite /srpre size_sub' /#.
++ split; last smt().
+  by move=> Hpre; rewrite size_nseq; smt(nth_u8zeros).
++ rewrite ler_maxr; first smt(size_ge0).
+  move=> H; split; last smt().
+  move=> Hpre; split.
+   by rewrite srpre_next; smt(size_ge0).
+  rewrite u8prefAbsorbP => i; rewrite size_nseq size_sub' nth_u8zeros.
+  case: (0 <= i < size lw) => C; last smt().
+  by rewrite nth_out /#.
+split; last smt().
+by move=> ?; rewrite sub0 size_nseq; smt(size_ge0 nth_u8zeros).
+qed.
+
+lemma asubread_cat (buf:W8.t A.t) off lw1 lw2 (cur at dlt len tb:int) at1 dlt1 len1 tb1 at2 dlt2 len2 tb2:
+ asubread buf off lw1 cur at dlt len tb at1 dlt1 len1 tb1 =>
+ asubread buf off lw2 (cur+size lw1) at1 dlt1 len1 tb1 at2 dlt2 len2 tb2 =>
+ asubread buf off (lw1++lw2) cur at dlt len tb at2 dlt2 len2 tb2.
+proof.
+rewrite /asubread => /= [#]H1 Hat1 Hdlt1 Hlen1 Htb1.
+move => /= [#]H2 Hat2 Hdlt2 Hlen2 Htb2.
+split; last first.
+ by rewrite size_cat srat_add; smt(size_ge0).
+move => Hpre; move:(Hpre).
+have Hl: sub buf (off + dlt1) len1 = srl (size lw1) cur at (sub buf (off + dlt) len).
+ smt(size_ge0 drop_sub). 
+by apply (srspec_cat lw1 lw2 cur at (sub buf (off + dlt) len) len tb) => // /#.
+qed.
+
+op asubwrite (a a2: W8.t A.t) off lw (dlt len:int) dlt2 len2 =
+ a2 = A.fill (fun i => lw.[i-off+dlt]) (off+dlt) len a
+ /\ dlt2 = dlt + min (size lw) (max 0 len)
+ /\ len2 = len - min (size lw) (max 0 len).
+
+lemma asubwrite_cat a a1 a2 off lw1 lw2 dlt len dlt1 len1 dlt2 len2:
+ asubwrite a a1 off lw1 dlt len dlt1 len1 =>
+ asubwrite a1 a2 off lw2 dlt1 len1 dlt2 len2 =>
+ asubwrite a a2 off (lw1++lw2) dlt len dlt2 len2.
+proof.
+move=> />; split; last smt(size_ge0 size_cat).
+rewrite !fillE tP => i Hi; rewrite !initiE //= initiE //=.
+case: (off + dlt <= i < off + dlt + len) => C; last first.
+ by rewrite ifF; first smt(size_ge0).
+rewrite nth_cat.
+case: (i - off + dlt < size lw1) => C1.
+ rewrite ifF //.
+ admit.
+rewrite ifT //.
+ admit.
+congr.
+admit.
+qed.
+
+
+
 module MM = {
   proc __a_ilen_read_upto8_at (buf:W8.t A.t, offset:int, dELTA:int,
                                lEN:int, tRAIL:int, cUR:int, aT:int) : 
@@ -293,7 +1389,7 @@ module MM = {
     var w:W64.t;
     var t16:W64.t;
     var t8:W64.t;
-    if ((((aT < cUR) \/ ((cUR + 8) <= aT)) \/ ((lEN = 0) /\ (tRAIL = 0)))) {
+    if ((((lEN < 0) \/ (aT < cUR) \/ ((cUR + 8) <= aT)) \/ ((lEN = 0) /\ (tRAIL = 0)))) {
       w <- (W64.of_int 0);
     } else {
       if ((8 <= lEN)) {
@@ -363,7 +1459,7 @@ module MM = {
     var w:W128.t;
     var t64_0:W64.t;
     var t64_1:W64.t;
-    if ((((aT < cUR) \/ ((cUR + 16) <= aT)) \/ ((lEN = 0) /\ (tRAIL = 0)))) {
+    if ((((lEN < 0) \/ (aT < cUR) \/ ((cUR + 16) <= aT)) \/ ((lEN = 0) /\ (tRAIL = 0)))) {
       w <- (set0_128);
     } else {
       if ((16 <= lEN)) {
@@ -397,7 +1493,7 @@ module MM = {
     var w:W256.t;
     var t128_0:W128.t;
     var t128_1:W128.t;
-    if ((((aT < cUR) \/ ((cUR + 32) <= aT)) \/ ((lEN = 0) /\ (tRAIL = 0)))) {
+    if ((((lEN < 0) \/ (aT < cUR) \/ ((cUR + 32) <= aT)) \/ ((lEN = 0) /\ (tRAIL = 0)))) {
       w <- (set0_256);
     } else {
       if (((aT = cUR) /\ (32 <= lEN))) {
@@ -431,7 +1527,7 @@ module MM = {
     var aT8:int;
     var w:W64.t;
     var t128:W128.t;
-    if ((((aT < cUR) \/ ((cUR + 8) <= aT)) \/ ((lEN = 0) /\ (tRAIL = 0)))) {
+    if ((((lEN < 0) \/ (aT < cUR) \/ ((cUR + 8) <= aT)) \/ ((lEN = 0) /\ (tRAIL = 0)))) {
       w256 <- (set0_256);
     } else {
       if ((8 <= lEN)) {
@@ -788,74 +1884,235 @@ by islossless.
 lemma a_rlen_write_upto8_ll: islossless MM.__a_rlen_write_upto8
 by islossless.
 
-
-
-lemma sub0 (buf: W8.t A.t) off:
- sub buf off 0 = [].
-proof. by rewrite -size_eq0 size_sub /#. qed.
-
-
-
-op subread_pre cur at off dlt len tb =
- 0 <= cur /\ 0 <= at /\ 0 <= off /\ 0 <= dlt /\ 0 <= len /\ 0 <= tb < 256 /\
- off + dlt + len <= _ASIZE /\
- at + len + b2i (tb<>0) <= 200 /\
- (cur <= at || len=0 /\ tb=0).
-
-
-lemma nth_bytes_at sz cur at buf off dlt len tb i:
- 0 <= sz =>
- subread_pre cur at off dlt len tb =>
- nth W8.zero (bytes_at sz cur at (A.sub buf (off+dlt) len++[W8.of_int tb])) i
- = if 0 <= at-cur <= i < sz
-   then nth W8.zero (sub buf (off+dlt) len++[W8.of_int tb]) (cur+i-at)
-   else W8.zero.
+lemma a_ilen_read_upto8_at_h _buf _off _dlt _len _tb _cur _at:
+ (* 0 <= _len => *)
+ hoare [
+ MM.__a_ilen_read_upto8_at
+ : buf=_buf /\ offset=_off /\ dELTA=_dlt /\ lEN=_len /\ tRAIL=_tb /\ cUR=_cur /\ aT=_at
+ /\ 0 <= _len
+ ==> asubread _buf _off (u64bytes res.`5) _cur _at _dlt _len _tb res.`4 res.`1 res.`2 res.`3
+ ].
 proof.
-move=> /> ??????????[H|H].
-+ case: (0 <= i < sz) => C; last first.
-   by rewrite nth_out 1:size_bytes_at // ifF /#.
-  case: (i < at-cur) => C1.
-   rewrite ifF 1:/# nth_take 1..2:/# nth_cat ifT.
-    by rewrite size_drop // !size_cat size_sub //= size_nseq /#.
-   rewrite nth_drop 1..2:/# nth_cat ifT 1:size_nseq 1:/#.
-   by rewrite nth_nseq 1:/#.
-  rewrite ifT 1:/# nth_take 1..2:/# nth_cat.
-  rewrite size_drop 1:/# !size_cat size_sub //= size_nseq //=.
-  case: (i < at + (len + 1) - cur) => C2.
-   by rewrite ifT 1:/# nth_drop 1..2:/# nth_cat size_nseq ifF /#.
-  rewrite ifF 1:/# nth_nseq 1:/# nth_out //.
-  by rewrite size_cat size_sub /#.
-move=> []->->; rewrite sub0 /= /bytes_at.
-case: (0 <= i < sz) => C; last first.
- rewrite nth_out // size_take // size_cat.
- by rewrite size_drop // size_cat !size_nseq /#.
-rewrite nth_take 1..2:/# nth_cat nth_drop 1..2:/#.
-rewrite nth_cat !size_drop // !size_cat !size_nseq /=.
-case: (cur+i<at) => C1.
- by rewrite !nth_nseq /#.
-rewrite nth_out 1:size_nseq 1:/#.
-by rewrite nth_nseq /#.
+proc; simplify.
+if => //.
+ auto => |> Hlen_ge0 H; apply asubread0.
+  by rewrite size_to_list u64bytes0.
+ by rewrite size_to_list /#.
+sp; if => //.
+ (* 8 <= lEN *)
+ wp; ecall (SHLQ_h w (aT-cUR)); auto => |> *.
+ split; first smt().
+ move=> ??.
+ admit (*by apply asubread_u64.*).
+
+conseq (: _cur <= _at < _cur+8 /\ 0 <= _len < 8 /\ (_len<>0 \/ _tb<>0) 
+         /\ buf=_buf /\ offset=_off /\ 0 <= _len /\ cUR=_cur /\ tRAIL=_tb
+         /\ dELTA=_dlt /\ lEN=_len /\ aT=_at==> _).
+ by move => /> /#.
+
+pose n0 := min (_cur + 8 - _at) (_len %/ 4 * 4).
+seq 1: ( #[:8]pre
+       /\ asubread _buf _off (u64bytes w) _cur _at _dlt (_len %/ 4 * 4) 0 aT dELTA lEN 0 
+       /\ dELTA = _dlt+n0 /\ lEN = _len - n0 /\ aT=_at+n0).
+ if => //.
+  (* 4 <= lEN  *)
+  wp; ecall (SHLQ_h w (aT-cUR)); auto => /> *.
+  split; first smt().
+  move=> ??.
+  rewrite /n0.
+  have ->: _len %/ 4 * 4 = 4 by smt().
+  have ->: (_dlt + if _cur + 8 <= _at + 4 then _cur + 8 - _at else 4)
+          = _dlt + min (_cur+8-_at) 4 by smt().
+  have ->: (if _cur + 8 <= _at + 4 then _cur + 8 else _at + 4)
+          = _at + min (_cur+8-_at) 4 by smt().
+  split.
+   admit (*by apply (subread_u32 (min (_cur+8-_at) 4) _buf _off _dlt _cur _at _ _); smt().*).
+  smt().
+ auto => /> ??????.
+ rewrite /n0 size_to_list.
+ have ->: _len%/4*4 = 0 by smt().
+ rewrite ler_minr 1:/# /=.
+ admit (*by apply subread_spec_empty8.*).
+
+pose n1 := min (_cur+8-_at) (_len %/ 2 * 2).
+exlim aT => at1; exlim lEN => len1; exlim dELTA => dlt1.
+conseq (: _cur <= _at < _cur+8 /\ 0 <= _len < 8 /\ (_len<>0 \/ _tb<>0) 
+         /\ buf=_buf /\ offset=_off /\ 0 <= _len /\ cUR=_cur
+         /\ tRAIL=_tb /\ dELTA=dlt1 /\ lEN=len1 /\ aT=at1
+         /\ asubread _buf _off (u64bytes w) _cur _at _dlt (_len%/4*4) 0 
+              at1 dlt1 (_len %/ 4 * 4 - n0) 0
+         /\ dlt1=_dlt+n0 /\ len1=_len-n0 /\ at1=_at+n0
+         ==> _).
+ by move => /> *; rewrite size_to_list /srincr /n0 /#. 
+
+seq 1: ( #[/:10]pre
+/\ asubread _buf _off (u64bytes w) _cur _at _dlt (_len %/ 2 * 2) 0
+     aT dELTA (_len%/2*2-n1) 0
+/\ dELTA=_dlt+n1 /\ lEN=_len-n1 /\ aT=_at+n1).
+ if => //.
+  (* 2 <= lEN *)
+  wp; ecall (SHLQ_h t16 (aT-cUR)); auto => |> ?????? H1 ?? *.
+  split; first smt(). 
+  move=> ??; split.
+   rewrite -!addzA.
+   have ->: (n0 + if _cur + 8 <= _at + (n0 + 2) then _cur + (8 - (_at + n0)) else 2)=n1 by smt().
+   have ->: (if _cur + 8 <= _at + (n0 + 2) then _cur + 8 else _at + (n0 + 2))=_at+n1 by smt().
+   rewrite (addzA _at).
+   admit (*by apply (subread_w4_u16 n1 _buf _off _ _ _ _ _ _ _ _ _ _ _ _ H1); smt().*).
+  smt().
+ auto => |> &m ?????H.
+ rewrite negb_and; move => [?|?].
+  have En0: n0 = _cur+8-_at by smt().
+  have En1: n1 = n0 by smt().
+  split.
+   rewrite En1 {2}En0.
+   admit (*by apply (subread_w4_ahead _buf _off _ _ _ _ _ _ _ _ _ _ _ H); smt().*).
+  smt().
+ have ->: (_len %/ 2 * 2) = (_len %/ 4 * 4) by smt().
+ have ->: n1 = n0 by smt().
+ split; first smt().
+ smt(). 
+
+pose n2 := min (_cur+8-_at) _len.
+exlim aT => at2; exlim lEN => len2; exlim dELTA => dlt2.
+conseq (: _cur <= _at < _cur+8 /\ 0 <= _len < 8 /\ (_len<>0 \/ _tb<>0) 
+         /\ buf=_buf /\ offset=_off /\ 0 <= _len /\ cUR=_cur
+         /\ tRAIL=_tb /\ dELTA=dlt2 /\ lEN=len2 /\ aT=at2
+         /\ asubread _buf _off (u64bytes w) _cur _at _dlt (_len%/2*2) 0
+             at2 dlt2 (_len %/ 2 * 2 - n1) 0
+         /\ dlt2=_dlt+n1 /\ len2=_len-n1 /\ at2=_at+n1
+         ==> _).
+ by move => />. 
+
+seq 1: ( #[/:10]pre
+       /\ asubread _buf _off (u64bytes w) _cur _at _dlt _len 0
+                        aT dELTA (_len-n2) 0
+       /\ dELTA=_dlt+n2 /\ lEN=_len-n2 /\ aT=_at+n2).
+ if => //.
+  (* 1 <= lEN *)
+  wp; ecall (SHLQ_h t8 (aT-cUR)); auto => |> ?????? H1??*.
+  split; first smt(). 
+  move=> ??; split.
+   rewrite -!addzA.
+   have ->: n1+1=n2 by smt().
+   rewrite (addzA _at).
+   admit (*by apply (subread_w2_u8 n2 _buf _off _ _ _ _ _ _ _ _ _ _ _ _ H1); smt().*).
+  smt().
+ auto => |> &m ?????H.
+ rewrite negb_and; move => [?|?].
+  have En1: n1 = _cur+8-_at by smt().
+  have En2: n2 = n1 by smt().
+  split.
+   rewrite En2 {2}En1.
+   admit (*by apply (subread_w2_ahead _buf _off _ _ _ _ _ _ _ _ _ _ _ H); smt().*).
+  smt().
+ have ->: _len = _len %/ 2 * 2 by smt().
+ have ->: n2 = n1 by smt().
+ split; first smt().
+ smt(). 
+
+if => //.
+ auto => |> &m ?????H??.
+ admit (*by apply subread_w8_trail => /#.*).
+auto => |> &m ?????H; rewrite negb_and => [[C|C]].
+ admit (*by apply subread_w8_trail_ahead => /#.*).
+smt().
 qed.
 
 
+lemma a_ilen_read_upto16_at_h _buf _off _dlt _len _tb _cur _at:
+ (* 0 <= _len => *)
+ hoare [
+ MM.__a_ilen_read_upto16_at
+ : buf=_buf /\ offset=_off /\ dELTA=_dlt /\ lEN=_len /\ tRAIL=_tb /\ cUR=_cur /\ aT=_at
+ ==> asubread _buf _off (u128bytes res.`5) _cur _at _dlt _len _tb res.`4 res.`1 res.`2 res.`3
+ ].
+proof.
+proc; simplify.
 
-op subread_spec
- (size: int)
- (buf: W8.t A.t) (off dlt len tb cur at: int)
- (dlt' len' tb' at': int) (w: W8.t list)
- : bool =
- 0 <= size =>
- subread_pre cur at off dlt len tb =>
- subread_pre (cur+size) at' off dlt' len' tb'
- /\ w = bytes_at size cur at (sub buf (off+dlt) len ++ [W8.of_int tb])
- /\ at+len+b2i(tb<>0)=at'+len'+b2i(tb'<>0)
- /\ (tb'=tb || len'=0 && tb'=0)
- /\ dlt+len = dlt'+len'
- /\ at' = max at
-              (min (cur+size)
-                   (at+len+b2i (tb<>0)))
- /\ len' = max 0 (len - (max 0 (cur+size-at))).
+if => //.
+ auto => |> H.
+ apply asubread0.
+  admit.
+ by rewrite size_to_list /#.
 
+(* 16 <= lEN *)
+if => //.
+ wp; ecall (SHLDQ_h w (aT-cUR)); auto => |> *.
+ split; first smt().
+ move=> ??.
+ admit (*by apply (subread_u128 _buf _off _dlt _len _trail _cur _at _).*).
+
+(* lEN < 16 *)
+if => //.
+ (* CUR+8 <= AT *)
+ wp; ecall(a_ilen_read_upto8_at_h buf offset dELTA lEN tRAIL (cUR+8) aT); auto => |>.
+ rewrite !negb_or negb_and => |> ????????; split; first smt().
+ move=> _ [dlt0 len0 tb0 at0 w0] /= H.
+admit (*
+ have H0:= subread_spec_ahead8 _buf _off _dlt _len _trail _cur _at _;first  smt().
+ rewrite -zeroextu128_zero -u64bytes_cat.
+ by apply (subread_spec_cat 8 8 _ _ _ _ _ _ _ _ _ _ _ _ _ _ _ _ _ _ _ H0).*).
+
+wp; ecall(a_ilen_read_upto8_at_h buf offset dELTA lEN tRAIL (cUR+8) aT).
+wp; ecall(a_ilen_read_upto8_at_h buf offset dELTA lEN tRAIL cUR aT).
+auto => |>; rewrite !negb_or negb_and. 
+move => |>*; split; first smt().
+move => _ []dlt0 len0 tb0 at0 w0 |> H0.
+split; first smt().
+move=> _ []dlt1 len1 tb1 at1  w2 /= H1.
+rewrite -u64bytes_cat.
+by apply (asubread_cat _ _ _ _ _ _ _ _ _ _ _ _ _ _ _ _ _ H0).
+qed.
+
+phoare a_ilen_read_upto16_at_ph _buf _off _dlt _len _tb _cur _at:
+ [ MM.__a_ilen_read_upto16_at
+ : buf=_buf /\ offset=_off /\ dELTA=_dlt /\ lEN=_len /\ tRAIL=_tb /\ cUR=_cur /\ aT=_at
+ ==> asubread _buf _off (u128bytes res.`5) _cur _at _dlt _len _tb res.`4 res.`1 res.`2 res.`3
+ ] = 1%r.
+proof.
+by conseq a_ilen_read_upto16_at_ll
+          (a_ilen_read_upto16_at_h _buf _off _dlt _len _tb _cur _at).
+qed.
+
+hoare a_ilen_read_upto32_at_h _buf _off _dlt _len _tb _cur _at:
+ MM.__a_ilen_read_upto32_at
+ : buf=_buf /\ offset=_off /\ dELTA=_dlt /\ lEN=_len /\ tRAIL=_tb /\ cUR=_cur /\ aT=_at
+ ==> asubread _buf _off (u256bytes res.`5) _cur _at _dlt _len _tb res.`4 res.`1 res.`2 res.`3.
+proof.
+proc; simplify.
+
+if => //.
+ auto => |> H. 
+ apply asubread0.
+  admit.
+ by rewrite size_to_list /#.
+
+(* 32 <= lEN *)
+sp; if => //.
+ auto => |> ??.
+admit(* by apply subread_u256.*).
+
+(* lEN < 16 *)
+if => //.
+ (* CUR+16 <= AT *)
+ wp; ecall(a_ilen_read_upto16_at_h buf offset dELTA lEN tRAIL (cUR+16) aT); auto => |>.
+ rewrite !negb_or negb_and => |> ??????? [dlt0 len0 tb0 at0 w0] /= H.
+admit(*
+ have H0:= subread_spec_ahead16 _buf _off _dlt _len _trail _cur _at _;first  smt().
+ rewrite -zeroextu256_zero -u128bytes_cat.
+ by apply (subread_spec_cat 16 16 _ _ _ _ _ _ _ _ _ _ _ _ _ _ _ _ _ _ _ H0) => //.*).
+wp; ecall(a_ilen_read_upto16_at_h buf offset dELTA lEN tRAIL (cUR+16) aT).
+wp; ecall(a_ilen_read_upto16_at_h buf offset dELTA lEN tRAIL cUR aT).
+auto => |>.
+rewrite !negb_or negb_and. 
+move => ???[]dlt0 len0 tb0 at0 w0 |> H0 []dlt1 len1 tb1 at1 w1 /= H1.
+rewrite -u128bytes_cat.
+by apply (asubread_cat _ _ _ _ _ _ _ _ _ _ _ _ _ _ _ _ _ H0 _).
+qed.
+
+
+(*
 lemma subread_specP N buf off dlt len trail cur at dlt' at' w':
  0 <= N =>
  cur <= at =>
@@ -1041,54 +2298,7 @@ case: (tb=0) => Ctb.
  by rewrite Ctb /#.
 by rewrite ifF /#.
 qed.
-
-lemma subread_spec_cat N1 N2 buf off dlt dlt' dlt'' len len' len'' tb tb' tb'' cur at at' at'' w' w'':
- 0 <= N1 => 0 <= N2 =>
- subread_spec N1 buf off dlt len tb cur at dlt' len' tb' at' w' =>
- subread_spec N2 buf off dlt' len' tb' (cur+N1) at' dlt'' len'' tb'' at'' w'' =>
- subread_spec (N1+N2) buf off dlt len tb cur at dlt'' len'' tb'' at'' (w'++w'').
-proof.
-move=> HN1 HN2 H1 H2 _ Hpre1.
-move: (H1 HN1 Hpre1) => []Hpre2 {H1} [#]->*.
-move: (H2 HN2 Hpre2) => []Hpre3 {H2} [#]->*.
-split; first smt().
-split; last smt().
-apply (eq_from_nth W8.zero).
- by rewrite size_cat !size_bytes_at /#.
-rewrite size_cat !size_bytes_at 1..2:/# => i Hi.
-rewrite nth_cat size_bytes_at 1:/#.
-case: (i<N1) => Ci.
- by rewrite !nth_bytes_at /#.
-case: (at<cur) => Hcur.
- by rewrite !nth_bytes_at /#.
-rewrite !nth_bytes_at 1..4:/#.
-rewrite (:cur+N1+(i-N1)-at'=cur+i-at') 1:/#.
-case: (at'<cur+N1) => Cat'.
- have ->: len'=0 by smt().
- have ->: tb'=0 by smt().
- have ?: len < N1 by smt().
- rewrite ifF 1:/# ifT 1:/#.
- by rewrite nth_out // size_cat size_sub /#.
-case: (at<=cur+N1) => Cat.
- rewrite ifT 1:/# ifT 1:/#.
- have : at'=cur+N1 by smt().
- move => />.
- case: (tb'=tb) => Ctb.
-  rewrite nth_cat ?size_sub 1:/#.
-  case: (cur + i - (cur + N1) < len - (cur + N1 - at)) => CC.
-   by rewrite nth_sub 1:/# nth_cat ?size_sub 1:/# ifT 1:/# nth_sub 1:/# /#.
-  case: (tb=0) => Etb.
-   by rewrite nth_cat ?size_sub 1:/# ifF 1:/# /#.
-  rewrite nth_cat ?size_sub 1:/#.
-  case: (cur + i - at < len) => ?.
-   by rewrite nth_sub /#.
-  smt().
- have ->: len'=0 by smt().
- have ->: tb'=0 by smt().
- rewrite sub0 /= nth_cat size_sub 1:/#.
- by rewrite ifF 1:/# nth_out /#.
-smt().
-qed.
+*)
 
 
 lemma get128_bytes (buf: W8.t A.t) off k:
@@ -1167,6 +2377,7 @@ case: (i<k) => // C.
 by rewrite nth_sub /#.
 qed.
 
+(*
 lemma subread_u128 _buf _off _dlt _len _trail _cur _at:
  16 <= _len =>
  0 <= _at-_cur < 16 =>
@@ -1432,7 +2643,9 @@ split.
  by rewrite !nth_cat !size_sub /#.
 smt().
 qed.
+*)
 
+(*
 lemma a_ilen_read_upto8_at_h _buf _off _dlt _len _trail _cur _at:
  (* 0 <= _len => *)
  hoare [
@@ -1702,9 +2915,7 @@ proof.
 by conseq a_ilen_read_upto32_at_ll
           (a_ilen_read_upto32_at_h _buf _off _dlt _len _trail _cur _at).
 qed.
-
-
-
+*)
 
 
 lemma trunc_zext_u64_u128 w:
@@ -1725,20 +2936,751 @@ if => //=.
  auto => />.
  by move=> *; clear; circuit.
 sp; if => //=.
- inline*; auto => /> &m *; do (split => *).
- + smt().
- + smt().
- + rewrite /VPSLL_4u64 /VPBROADCAST_4u64 /= -iotaredE /=; congr => />.
-   by rewrite /W64.(`<<`) trunc_zext_u64_u128 of_uintK modz_small 1:/# of_uintK modz_small /#.
- + smt().
- + smt().
- + by rewrite /W64.(`<<`) trunc_zext_u64_u128; congr; congr.
+ inline*; auto => /> &m *; split.
+  move=> *; split; first smt().
+  split; first smt().
+  rewrite /VPSLL_4u64 /VPBROADCAST_4u64 /= -iotaredE /=; congr => />.
+  by rewrite /W64.(`<<`) trunc_zext_u64_u128 of_uintK modz_small 1:/# of_uintK modz_small /#.
+ move=> *; split; first smt().
+ split; first smt().
+ by rewrite /W64.(`<<`) trunc_zext_u64_u128; congr; congr.
 inline *.
 rcondf {1} 9; first by auto.
 rcondf {1} 9; first by auto.
 admitted.
 
 
+lemma fill_le0 f off len (buf: W8.t A.t):
+ len <= 0 =>
+ fill f off len buf = buf.
+proof.
+move=> H; rewrite fillE tP => i Hi.
+by rewrite initiE //= ifF 1:/#.
+qed.
 
 
+(*
+op subwrite_mpre n ptr len =
+ 0 <= n /\ 0 <= ptr /\ 0 <= len.
+
+op subwrite_mspec n mem ptr len l mem1 ptr1 len1 =
+ subwrite_mpre n ptr len =>
+ mem1 = stores mem ptr (take (min len 8) l)
+ /\ ptr1 = ptr + min len 8
+ /\ len1 = len - min len 8.
+
+op subwrite_apre n off dlt len =
+ 0 <= n /\ 0 <= off /\ 0 <= dlt /\ 0 <= len /\ off + dlt + min len n <= _ASIZE.
+
+op subwrite_aspec n (buf: W8.t A.t) off dlt len l buf1 dlt1 len1 =
+ subwrite_apre n off dlt len =>
+ buf1 = A.fill (fun i => nth W8.zero l (i-off+dlt)) (off+dlt) len buf
+ /\ dlt1 = dlt + min len 8
+ /\ len1 = len - min len 8.
+
+
+op subread_mpre cur at ptr len tb =
+ 0 <= cur /\ 0 <= at /\ 0 <= ptr /\ 0 <= len /\ 0 <= tb < 256 /\
+ at + len + b2i (tb<>0) <= 200 /\
+ (cur <= at || len=0 /\ tb=0).
+
+op reads len (m: global_mem_t) (a: address) = mkseq (fun i => m.[a+i]) len.
+
+op subread_mspec
+ (size: int)
+ mem (ptr len tb cur at: int)
+ (ptr' len' tb' at': int) (w: W8.t list)
+ : bool =
+ 0 <= size =>
+ subread_mpre cur at ptr len tb =>
+ subread_pre (cur+size) at' ptr' len' tb'
+ /\ w = bytes_at size cur at (reads len mem ptr) ++ [W8.of_int tb]
+ /\ at+len+b2i(tb<>0)=at'+len'+b2i(tb'<>0)
+ /\ (tb'=tb || len'=0 && tb'=0)
+ /\ dlt+len = dlt'+len'
+ /\ at' = max at
+              (min (cur+size)
+                   (at+len+b2i (tb<>0)))
+ /\ len' = max 0 (len - (max 0 (cur+size-at))).
+
+op subread_apre cur at off dlt len tb =
+ 0 <= cur /\ 0 <= at /\ 0 <= off /\ 0 <= dlt /\ 0 <= len /\ 0 <= tb < 256 /\
+ off + dlt + len <= _ASIZE /\
+ at + len + b2i (tb<>0) <= 200 /\
+ (cur <= at || len=0 /\ tb=0).
+
+op subread_aspec
+ (size: int)
+ (buf: W8.t A.t) (off dlt len tb cur at: int)
+ (dlt' len' tb' at': int) (w: W8.t list)
+ : bool =
+ 0 <= size =>
+ subread_pre cur at off dlt len tb =>
+ subread_pre (cur+size) at' off dlt' len' tb'
+ /\ w = bytes_at size cur at (sub buf (off+dlt) len ++ [W8.of_int tb])
+ /\ at+len+b2i(tb<>0)=at'+len'+b2i(tb'<>0)
+ /\ (tb'=tb || len'=0 && tb'=0)
+ /\ dlt+len = dlt'+len'
+ /\ at' = max at
+              (min (cur+size)
+                   (at+len+b2i (tb<>0)))
+ /\ len' = max 0 (len - (max 0 (cur+size-at))).
+*)
+
+(* buf,delta,len = *)
+hoare a_ilen_write_upto8_h _buf _off _dlt _len _w:
+ MM.__a_ilen_write_upto8
+ : buf=_buf /\ offset=_off /\ dELTA=_dlt /\ lEN=_len /\ w = _w
+ ==> asubwrite _buf res.`1 _off (u64bytes _w) _dlt _len res.`2 res.`3.
+proof.
+proc; simplify.
+if => //=; last first.
+ auto => /> Hlen.
+ by rewrite fill_le0 1:/# size_to_list /#.
+if => //.
+ auto => /> _ ?; split.
+ rewrite tP => i Hi.
+ rewrite initiE // filliE // get8_set64_directE.
+admit (* 0 <= _off+_dlt *).
+admit (* 0 <= _off+_dlt <= ASIZE-8 *).
+case: (_off + _dlt <= i < _off + _dlt + 8) => ?.
+ rewrite ifT 1:/#.
+ admit.
+rewrite /get8 initiE // ifF. admit.
+smt().
+by rewrite size_to_list /#.
+
+(* seq 1: ( subwrite_spec buf (off+dlt) (len%/4*4) *)
+if => //.
+admitted.
+
+phoare a_ilen_write_upto8_ph _buf _off _dlt _len _w:
+ [ MM.__a_ilen_write_upto8
+ : buf=_buf /\ offset=_off /\ dELTA=_dlt /\ lEN=_len /\ w = _w
+ ==> asubwrite _buf res.`1 _off (u64bytes _w) _dlt _len res.`2 res.`3
+ ] = 1%r.
+proof. by conseq a_ilen_write_upto8_ll (a_ilen_write_upto8_h _buf _off _dlt _len _w). qed.
+
+
+
+hoare a_ilen_write_upto16_h _buf _off _dlt _len _w:
+ MM.__a_ilen_write_upto16
+ : buf=_buf /\ offset=_off /\ dELTA=_dlt /\ lEN=_len /\ w = _w
+ ==> asubwrite _buf res.`1 _off (u128bytes _w) _dlt _len res.`2 res.`3.
+proof.
+admitted.
+
+phoare a_ilen_write_upto16_ph _buf _off _dlt _len _w:
+ [ MM.__a_ilen_write_upto16
+ : buf=_buf /\ offset=_off /\ dELTA=_dlt /\ lEN=_len /\ w = _w
+ ==> asubwrite _buf res.`1 _off (u128bytes _w) _dlt _len res.`2 res.`3
+ ] = 1%r.
+proof. by conseq a_ilen_write_upto16_ll (a_ilen_write_upto16_h _buf _off _dlt _len _w). qed.
+
+hoare a_ilen_write_upto32_h _buf _off _dlt _len _w:
+ MM.__a_ilen_write_upto32
+ : buf=_buf /\ offset=_off /\ dELTA=_dlt /\ lEN=_len /\ w = _w
+ ==> asubwrite _buf res.`1 _off (u256bytes _w) _dlt _len res.`2 res.`3.
+proof.
+admitted.
+
+phoare a_ilen_write_upto32_ph _buf _off _dlt _len _w:
+ [ MM.__a_ilen_write_upto32
+ : buf=_buf /\ offset=_off /\ dELTA=_dlt /\ lEN=_len /\ w = _w
+ ==> asubwrite _buf res.`1 _off (u256bytes _w) _dlt _len res.`2 res.`3
+ ] = 1%r.
+proof. by conseq a_ilen_write_upto32_ll (a_ilen_write_upto32_h _buf _off _dlt _len _w). qed.
+
+
+
+
+(*.
+lemma sub_cat (buf: W8.t A.t) off dlt x y:
+  0 <= off =>
+  0 <= dlt =>
+  0 <= y =>
+  0 <= x =>
+  y <= x =>
+  sub buf (off + dlt) x =
+  sub buf (off + dlt) y ++
+  sub buf (off + dlt + y) (x-y).
+proof.
+move =>*.
+  pose l1 := sub buf (off + dlt) x.
+  pose l2 := sub buf (off + dlt) y ++
+             sub buf (off + dlt + y) (x-y).
+  rewrite (eq_from_nth witness l1 l2).
+  + rewrite size_cat !size_sub /#. rewrite size_sub 1:/# => i i_bnd.
+    + rewrite nth_cat size_sub 1:/# nth_sub 1:/#. 
+      case(i < y) => i_small; by rewrite nth_sub /#.
+   smt().
+qed.
+
+lemma aux a b c d e f:
+  0 <= a =>
+  0 <= b =>
+  0 <= c =>
+  a + b + min c f <= d =>
+  0 <= e < min c f =>
+    0 <= a + b + e < d.
+proof.
+  move => H0 H1 H2.
+  case(c < f) => c_small.
+  + rewrite !lez_minl 1:/# => *. split. smt(). move=> *. rewrite (ltr_le_trans (a+b+c)) /#.
+  + rewrite !lez_minr 1:/# => *. split. smt(). move=> *. rewrite (ltr_le_trans (a+b+f)) /#. 
+qed.
+    
+lemma u8_from_u64 x _w:
+  0 <= x =>
+  x < 8 =>
+  W8.of_int (W64.to_uint _w %/ 2 ^ (8*x)) = (_w \bits8 x).
+    proof.
+  move => *.
+  rewrite /(\bits8) (W8.ext_eq _ (W8.init(fun j=> _w.[x * 8 + j]))). move => x0 x0_bnd.
+  + rewrite /of_int /to_uint bs2int_div 1:/# -(cat_take_drop 8 (drop (8*x) (w2bits _w))).
+    rewrite -(bs2intD _ _ 8) 1:size_take 1:/# 1:size_drop 1:/# 1:size_w2bits 1:/#.
+    rewrite dvdz_modzDr 1:/# int2bs_mod.
+    have{1}->: 8 = size (take 8 (drop (8*x) (w2bits _w)))
+      by rewrite size_take 1:/# size_drop 1:/# size_w2bits /#.
+    rewrite bs2intK /bits2w !initE !ifT ..2:/# /= nth_take ..2:/# nth_drop ..2:/#.
+    rewrite get_w2bits /#. smt().
+  qed.
+
+lemma u16_from_u64 x i _w:
+  x <= i =>
+  i < x+2 => 
+  0 <= x =>
+  x < 6 =>
+  (W16.of_int (W64.to_uint _w %/ 2 ^ (8*x)) \bits8 i - x) = (_w \bits8 i).
+proof.
+  move => *.
+  rewrite /(\bits8) (W8.ext_eq _ (W8.init(fun j=> _w.[i * 8 + j]))). move => x0 x0_bnd.
+  + rewrite /of_int /to_uint bs2int_div 1:/# -(cat_take_drop 16 (drop (8*x) (w2bits _w))).
+    rewrite -(bs2intD _ _ 16) 1:size_take 1:/# 1:size_drop 1:/# 1:size_w2bits 1:/#.
+    rewrite !initE !ifT ..2:/# /= dvdz_modzDr 1:/# int2bs_mod.
+    have{1}->: 16 = size (take 16 (drop (8*x) (w2bits _w)))
+      by rewrite size_take 1:/# size_drop 1:/# size_w2bits /#.
+    rewrite bs2intK /bits2w !initE ifT 1:/# /= nth_take ..2:/# nth_drop ..2:/#.
+    rewrite get_w2bits /#. smt().
+qed.
+
+lemma u32_from_u64 i _w: 
+  0 <= i =>
+  i < 4 =>
+(W32.of_int (W64.to_uint _w) \bits8 i) = (_w \bits8 i).
+proof.
+  move => *.
+  rewrite /(\bits8) (W8.ext_eq _ (W8.init(fun j=> _w.[i * 8 + j]))). move => x0 x0_bnd.
+  + rewrite /of_int /to_uint initE ifT 1:/# -(cat_take_drop 32 (w2bits _w)).
+    rewrite -(bs2intD _ _ 32) 1:size_take 1:/# 1:size_w2bits 1:/# dvdz_modzDr 1:/#.
+    rewrite int2bs_mod /=. have{1}->: 32 = size (take 32 (w2bits _w))
+      by rewrite size_take 1:/# size_w2bits /#.
+    rewrite bs2intK /bits2w !initE ifT 1:/# /= nth_take ..2:/# get_w2bits /#. smt().
+qed.
+
+
+op subwrite_pre (off dlt len size :int) : bool =
+  0 <= off /\ 0 <= dlt /\ 0 <= len /\ 8 <= size /\ off + dlt + min len size <= _ASIZE.
+
+op subwrite_spec
+ w (size: int)
+ (buf: W8.t A.t) (off dlt len: int)
+ (buf': W8.t A.t) (dlt' len': int)
+ : bool =
+ subwrite_pre off dlt len size =>
+ subwrite_pre off dlt len size /\
+ sub buf' 0 (off + dlt) = 
+ sub buf 0 (off + dlt) /\
+ sub buf' (off + dlt) (min len size) = 
+ take (min len size) (W8u8.to_list w) /\
+ dlt' = dlt + min len size /\
+ len' = max 0 (len - size).
+
+
+lemma u64_from_u64 buf off dlt len size w:
+  subwrite_pre off dlt len size =>
+  sub (A.init (get8 (set64_direct (WA.init8 (A."_.[_]" buf)) (off + dlt) w))) (off + dlt)
+     (min len 8) =
+  take len (to_list w).
+proof.
+  rewrite /subwrite_pre => H0.
+  + rewrite /sub /to_list -map_take /iotared take_iota minrC.
+    pose f1:= (fun (i : int) => (A.init (get8 (set64_direct
+                (WA.init8 ("_.[_]" buf)) (off + dlt) w))).[ off + dlt + i]).
+    rewrite (eq_in_mkseq f1 (((\bits8) w))). move => i i_bnd.
+    + rewrite /f1 /get8 /set64_direct initE ifT 1:(aux off dlt len _ASIZE i size) ..5:/# /=.
+      rewrite initE ifT 1:(aux off dlt len _ASIZE i size) ..5:/# /= ifT /#. smt().
+qed.
+
+hoare a_ilen_write_upto8_at_h _buf _off _dlt _len _w:
+ MM.__a_ilen_write_upto8
+ : buf=_buf /\ offset=_off /\ dELTA=_dlt /\ lEN=_len /\ w = _w /\
+   subwrite_pre _off _dlt _len 8
+ ==> subwrite_spec _w 8 _buf _off _dlt _len res.`1 res.`2 res.`3.
+proof.
+proc. if => //=; last first.
++ auto => /> *. do split; 1..4: smt(); 2..: smt().
+  + have->: _len = 0 by smt(). rewrite /sub mkseq0 take0 /#.
+(* 8 <= len *)
+if => //=. auto => /> *. 
+  + do split; ..4: smt(); 3..: smt().
+    rewrite (eq_from_nth W8.zero _ (sub _buf 0 (_off + _dlt))).
+    + rewrite !size_sub /#.
+    + rewrite size_sub 1:/# => i i_bnd.
+      rewrite /l1 !nth_sub ..2:/# initE ifT 1:/# /get8 /set8 /set64_direct initE.
+      rewrite ifT 1:/# /= ifF 1:/# initE ifT /#. smt().
+    rewrite (u64_from_u64 _buf _off _dlt _len 8 _w) /#.
+(* 4 <= LEN < 8 *)
+case( 7 <= lEN).
++ rcondt 1. auto => /#.
+  rcondt 5. auto => /#.
+  rcondt 9. auto => /#.
+  auto => /> *. do split; ..4: smt(); 3..: smt().
+    rewrite (eq_from_nth W8.zero _ (sub _buf 0 (_off + _dlt))).
+    + rewrite !size_sub /#.
+    + rewrite size_sub 1:/# => i i_bnd.
+      rewrite /l1 !nth_sub ..2:/# initE ifT 1:/# /get8 /set16_direct /set32_direct.
+      rewrite /init8 /truncateu8 get_setE 1:/# ifF 1:/# initE ifT 1:/# initE ifT 1:/#.
+      rewrite /= initE ifT 1:/# /= ifF 1:/# initE ifT 1:/# initE ifT 1:/# initE.
+      rewrite ifT 1:/# /= ifF 1:/# initE /#. smt().
+  + rewrite /sub /set16_direct /to_list -map_take /iotared take_iota minrC lez_minr 1:/#.
+    rewrite /truncateu16 /set32_direct /truncateu32 (eq_in_mkseq _ ((\bits8) _w)).
+    move => i i_bnd /=. rewrite /get8 /init8 initE ifT 1:/# /=.
+    case(i = 6) => i_max.
+    + rewrite get_setE 1:/# ifT 1:/# /truncateu8 !shr_div_le ..2:/# -divzMl ..2:/#.
+      have->: 2^16 * 2^32 = 2^(8 * 6) by smt(). rewrite u8_from_u64 /#.
+    case(4 <= i) => i_mid.
+    + rewrite get_setE 1:/# ifF 1:/# initE ifT 1:/# /= !initE !ifT ..2:/# /= ifT 1:/#.
+      rewrite !opprD !addrA shr_div_le 1:/#.
+      have->: _off + _dlt + i - _off - _dlt - 4 = i - 4 by smt().
+      have->: W32.modulus = 2^(8*4) by smt().
+      rewrite u16_from_u64 /#.
+    + rewrite get_setE 1:/# ifF 1:/# initE ifT 1:/# /= !initE !ifT ..2:/# /= ifF 1:/#.
+      rewrite initE ifT 1:/# initE ifT 1:/# !opprD initE.
+      rewrite ifT 1:/# /= ifT 1:/#. have->: _off + _dlt + i + ((-_off) - _dlt) = i by smt().
+      rewrite u32_from_u64 /#.  
+    smt().
+case(6 <= lEN).
++ rcondt 1. auto => /#.
+  rcondt 5. auto => /#.
+  rcondf 9. auto => /#.
+  auto => /> *. do split; ..4: smt(); 3..: smt().
+    rewrite (eq_from_nth W8.zero _ (sub _buf 0 (_off + _dlt))).
+    + rewrite !size_sub /#.
+    + rewrite size_sub 1:/# => i i_bnd.
+      rewrite /l1 !nth_sub ..2:/# initE ifT 1:/# /get8 /set16_direct /set32_direct.
+      rewrite /init8 initE ifT 1:/# /= ifF 1:/# initE ifT 1:/# initE ifT 1:/# initE.
+      rewrite ifT 1:/# /= initE ifF /#. smt().
+  + rewrite /sub /set16_direct /truncateu16 /to_list -map_take /iotared take_iota minrC.
+    rewrite lez_minr 1:/#/set32_direct /truncateu32 (eq_in_mkseq _ ((\bits8) _w)).
+    move => i i_bnd /=. rewrite /get8 /init8 initE ifT 1:/# /=.
+    case(4 <= i) => i_mid.
+    + rewrite initE ifT 1:/# /= !initE ifT 1:/# !opprD !addrA shr_div_le 1:/#.
+      have->: _off + _dlt + i - _off - _dlt - 4 = i - 4 by smt().
+      have->: W32.modulus = 2^(8*4) by smt().
+      rewrite u16_from_u64 /#.
+    + rewrite initE ifT 1:/# /= !initE ifF 1:/# !ifT..3:/# !opprD /= ifT 1:/# /=.
+      have->: _off + _dlt + i + ((-_off) - _dlt) = i by smt().
+      rewrite u32_from_u64 /#.
+    smt().
+case(5 <= lEN).
++ rcondt 1. auto => /#.
+  rcondf 5. auto => /#.
+  rcondt 5. auto => /#.
+  auto => />*. do split; ..4: smt(); 3..: smt().
+    rewrite (eq_from_nth W8.zero _ (sub _buf 0 (_off + _dlt))).
+    + rewrite !size_sub /#.
+    + rewrite size_sub 1:/# => i i_bnd.
+      rewrite /l1 !nth_sub ..2:/# initE ifT 1:/# /get8 /set16_direct /set32_direct.
+      rewrite /init8 get_setE 1:/# ifF 1:/# initE ifT 1:/# initE ifT 1:/# /= initE.
+      rewrite ifT 1:/# /= ifF 1:/# initE /#. smt().
+  + rewrite /sub /set16_direct /truncateu8 /to_list -map_take /iotared take_iota minrC.
+    rewrite lez_minr 1:/#  /set32_direct /truncateu32 (eq_in_mkseq _ ((\bits8) _w)).
+    move => i i_bnd /=. rewrite /get8 /init8 initE ifT 1:/# /=.
+    case(4 <= i) => i_mid.
+    + rewrite get_setE 1:/# ifT 1:/# shr_div_le 1:/#.
+      have->: 32 = 8 * 4 by smt(). rewrite u8_from_u64 /#.
+    + rewrite get_setE 1:/# ifF 1:/# initE ifT 1:/# /= !initE ifT 1:/# ifT 1:/# /= ifT 1:/#.
+      have->:  _off + _dlt + i - (_off + _dlt) = i by smt().
+      rewrite u32_from_u64 /#.  
+    smt().
+case(4 <= lEN).
+  rcondt 1. auto => /#.
+  rcondf 5. auto => /#.
+  rcondf 5. auto => /#.
+  auto => /> *. do split; ..4: smt(); 3..: smt().
+    rewrite (eq_from_nth W8.zero _ (sub _buf 0 (_off + _dlt))).
+    + rewrite !size_sub /#.
+    + rewrite size_sub 1:/# => i i_bnd.
+      rewrite /l1 !nth_sub ..2:/# initE ifT 1:/# /get8 /set32_direct.
+      rewrite /init8 initE ifT 1:/# /= ifF 1:/# initE /#. smt().
+  + rewrite /sub /set32_direct /truncateu32 /to_list -map_take /iotared take_iota minrC.
+    rewrite lez_minr 1:/#(eq_in_mkseq _ ((\bits8) _w)). move => i i_bnd /=.
+    rewrite /get8 /init8 initE ifT 1:/# /= initE ifT 1:/# /= ifT 1:/# opprD.
+    have->: _off + _dlt + i + ((-_off) - _dlt) = i by smt().
+    rewrite u32_from_u64 /#.
+    smt().
+rcondf 1. auto => /#.
+case(3 <= lEN).
+  rcondt 1. auto => /#.
+  rcondt 5. auto => /#.
+  auto => /> *. do split; ..4: smt(); 3..: smt().
+    rewrite (eq_from_nth W8.zero _ (sub _buf 0 (_off + _dlt))).
+    + rewrite !size_sub /#.
+    + rewrite size_sub 1:/# => i i_bnd.
+      rewrite /l1 !nth_sub ..2:/# initE ifT 1:/# /get8 /set16_direct /set32_direct.
+      rewrite /init8 get_setE 1:/# ifF 1:/# initE ifT 1:/# initE ifT 1:/# /= initE.
+      rewrite ifT 1:/# /= ifF 1:/# initE /#. smt().
+  + rewrite /sub /set16_direct /truncateu16 /to_list -map_take /iotared take_iota minrC.
+    rewrite lez_minr 1:/# /truncateu8 (eq_in_mkseq _ ((\bits8) _w)). move => i i_bnd /=.
+    rewrite /get8 /init8 initE ifT 1:/# /=.
+    case(2 <= i) => i_max.
+    + rewrite get_setE 1:/# ifT 1:/# shr_div_le 1:/#.
+      have->: 16 = 8 * 2 by smt(). rewrite u8_from_u64 /#.
+    + rewrite get_setE 1:/# ifF 1:/# initE ifT 1:/# !initE !ifT ..2:/#/= ifT 1:/#.
+      have->: _off + _dlt + i - (_off + _dlt) = i by smt().
+      rewrite (u16_from_u64 0 i _w) /#.
+    smt().
+case(2 <= lEN).
+  rcondt 1. auto => /#.
+  rcondf 5. auto => /#.
+  auto => /> *. do split; ..4: smt(); 3..: smt().
+    rewrite (eq_from_nth W8.zero _ (sub _buf 0 (_off + _dlt))).
+    + rewrite !size_sub /#.
+    + rewrite size_sub 1:/# => i i_bnd.
+      rewrite /l1 !nth_sub ..2:/# initE ifT 1:/# /get8 /set16_direct.
+      rewrite /init8 initE ifT 1:/# /= ifF 1:/# /= initE /#. smt().
+  + rewrite /sub /set16_direct /truncateu16 /to_list -map_take /iotared take_iota minrC.
+    rewrite lez_minr 1:/# (eq_in_mkseq _ ((\bits8) _w)). move => i i_bnd /=.
+    rewrite /get8 /init8 initE ifT 1:/# /= initE ifT 1:/# /= ifT 1:/# opprD.
+    have->: _off + _dlt + i + ((-_off) - _dlt) = i by smt().
+    rewrite (u16_from_u64 0 i _w) /#.
+    smt().
+rcondf 1. auto => /#.
+rcondt 1. auto => /#.
+auto => /> *. do split; ..4: smt(); 3..: smt().
+    rewrite (eq_from_nth W8.zero _ (sub _buf 0 (_off + _dlt))).
+    + rewrite !size_sub /#.
+    + rewrite size_sub 1:/# => i i_bnd.
+      rewrite /l1 !nth_sub ..2:/# initE ifT 1:/# /get8 /init8 get_setE 1:/# ifF 1:/#.
+      rewrite initE /#. smt().
+  rewrite /sub /truncateu8 /to_list -map_take /iotared take_iota minrC lez_minr 1:/#.
+  rewrite (eq_in_mkseq _ ((\bits8) _w)). move => i i_bnd /=.
+  rewrite initE ifT 1:/# /get8 /init8 get_setE 1:/# ifT 1:/# (u8_from_u64 0 _w) /#.
+  smt().
+qed.
+
+phoare a_ilen_write_upto8_at_ph _buf _off _dlt _len _w:
+ [ MM.__a_ilen_write_upto8
+ : buf=_buf /\ offset=_off /\ dELTA=_dlt /\ lEN=_len /\ w = _w /\
+   subwrite_pre _off _dlt _len 8
+ ==> subwrite_spec _w 8 _buf _off _dlt _len res.`1 res.`2 res.`3] = 1%r.
+proof.
+by conseq a_ilen_write_upto8_ll
+          (a_ilen_write_upto8_at_h _buf _off _dlt _len _w).
+qed.
+
+op subwriteu128_spec 
+  (w : W128.t) (size : int) 
+  (buf : W8.t A.t) (off dlt len : int)
+  (buf' : W8.t A.t) (dlt' len' : int) : bool =
+  subwrite_pre off dlt len size =>
+  subwrite_pre off dlt len size /\
+  sub buf' 0 (off + dlt) = sub buf 0 (off + dlt) /\
+  sub buf' (off + dlt) (min len size) = take len (to_list w) /\
+  dlt' = dlt + min len size /\ len' = max 0 (len - size).
+
+lemma u128_from_u128 buf off dlt len size w:
+  size = 16 =>
+  subwrite_pre off dlt len size =>
+  sub (A.init (get8 (set128_direct (WA.init8 (A."_.[_]" buf)) (off + dlt) w))) (off + dlt)
+     (min len 16) =
+  take len (to_list w).
+proof.
+  rewrite /subwriteX_pre => H0 *.
+  + rewrite /sub /to_list -map_take /iotared take_iota minrC.
+    rewrite (eq_in_mkseq _ (((\bits8) w))). move => i i_bnd.
+    + rewrite /get8 /set128_direct /= initE ifT 1:(aux off dlt len _ASIZE i size) ..5:/# /=.
+      rewrite initE ifT 1:(aux off dlt len _ASIZE i size) ..5:/# /= ifT /#. smt().
+qed.
+
+
+lemma set_highu64 _len _w:
+  take (_len - 8) (W8u8.to_list (truncateu64 (VPUNPCKH_2u64 _w _w))) =
+          take (_len - 8) (drop 8 (to_list _w)).
+proof.
+  move => *.
+  pose l1:= W8u8.to_list (truncateu64 (VPUNPCKH_2u64 _w _w)).
+  pose l2:= drop 8 (W16u8.to_list _w).
+  congr. rewrite (eq_from_nth W8.zero l1 l2).
+  + rewrite size_drop 1:/# !size_to_list /#.
+  + rewrite size_to_list => i i_bnd.
+    rewrite nth_drop ..2:/# /l1 /to_list !nth_to_list_in ..2:/#.
+    rewrite /truncateu64 /VPUNPCKH_2u64 /interleave_gen /get_hi_2u64 /=.
+    rewrite /of_int /to_uint bs2int_mod 1:/#.
+    have{1}->: 64 = size (take 64 (w2bits (pack2 [_w \bits64 1; _w \bits64 1]))).
+      by rewrite size_take 1:/# size_w2bits /#.
+    rewrite bs2intK (W8.ext_eq _ (_w \bits8 8 + i)). move => x0 x0_bnd.
+  + rewrite /pack2_t /bits2w /w2bits take_mkseq 1:/# /= /(\bits8) /= initE ifT 1:/#/=.
+    rewrite initE ifT 1:/# /= nth_mkseq 1:/# initE ifT 1:/# /(\bits64) /=.
+    rewrite /of_list initE ifT 1:/# /= ifT 1:/# !initE !ifT /#. smt().
+  smt().
+qed.
+
+lemma set_lowu64 buf off dlt len w:
+  0 <= off =>
+  0 <= dlt =>
+  0 <= len =>
+  off + dlt + 8 <= _ASIZE =>
+  sub (A.init (get8 (set64_direct (WA.init8 (A."_.[_]" buf)) (off + dlt) 
+  (MOVV_64 (truncateu64 w))))) (off + dlt) 8 =
+  take 8 (W16u8.to_list w).
+proof.
+ move =>*.
+ pose l1:= sub (A.init (get8 (set64_direct (WA.init8 ("_.[_]" buf)) (off + dlt) 
+           (MOVV_64 (truncateu64 w))))) (off + dlt) 8.
+  pose l2:= take 8 (W16u8.to_list w).
+  rewrite (eq_from_nth W8.zero l1 l2).
+  + rewrite size_mkseq size_take 1:/# size_to_list /#.
+  + rewrite size_mkseq lez_maxr 1:/# => i i_bnd.
+    rewrite nth_mkseq 1:/# /= initE ifT 1:/# /get8 /set64_direct.
+    rewrite initE ifT 1:/# /= ifT 1:/# /MOVV_64 /truncateu64.
+    have->: off + dlt + i - (off + dlt) = i by smt().
+    rewrite nth_take ..2:/# (W8.ext_eq _ (W16u8.to_list w).[i]). move => x x_bnd.
+    + rewrite nth_to_list /(\bits8) !initE !ifT ..2:/# /= /of_int /to_uint.
+      rewrite bs2int_mod 1:/#. 
+      have{1}->:64=size (take 64 (w2bits w))by rewrite size_take 1:/# size_w2bits /#.
+      rewrite bs2intK get_bits2w 1:/# nth_take ..2:/# get_w2bits /#.
+      smt().
+    smt().
+qed.
+
+
+hoare a_ilen_write_upto16_at_h _buf _off _dlt _len _w:
+ MM.__a_ilen_write_upto16
+ : buf=_buf /\ offset=_off /\ dELTA=_dlt /\ lEN=_len /\ w = _w /\
+   subwrite_pre _off _dlt _len 16
+ ==> subwriteu128_spec _w 16 _buf _off _dlt _len res.`1 res.`2 res.`3.
+proof.
+proc.
+if => //=; first last.
+auto => /> *. rewrite /subwrite_pre.
+  do split; ..4:smt(); 2..:smt().
+  + rewrite /sub /to_list -map_take /iotared take_iota minrC.
+    rewrite (eq_in_mkseq _ (((\bits8) _w))) /#.
+(*16 <= lEN *)
+if => //=.
+  auto => /> *. do split; ..4:smt(); 3..:smt().
+    rewrite (eq_from_nth W8.zero _ (sub _buf 0 (_off + _dlt))).
+    + rewrite !size_sub /#.
+    + rewrite size_sub 1:/# => i i_bnd.
+      rewrite /l1 !nth_sub ..2:/# initE ifT 1:/# /get8 /set8 /set128_direct initE.
+      rewrite ifT 1:/# /= ifF 1:/# initE ifT /#. smt().
+  rewrite (u128_from_u128 _ _ _ _ 16) /#. 
+(* 8 <= lEN *)
+case(8 <= lEN). 
+  rcondt 1. auto => /#.
+  ecall(a_ilen_write_upto8_at_h buf offset dELTA lEN t64). 
+  auto => /> H0 H1 H2 H3 H4 H5 H6. split; first by smt().
+  rewrite /subwrite_spec =>H7 H8 H9 H10 result _H0 _H1.
+  move: _H0. rewrite /subwrite_pre H7 H8 H9 H10 implyTb !addrA=> [#]?????.
+  have->: _off + _dlt + 8 - 8 = _off + _dlt by smt().
+  rewrite lez_minl 1:/# => h0 h1 h2 h3.
+  rewrite h2 h3. do split; ..3: smt(); 3..: smt().
+  move: h0. rewrite !(sub_cat _ 0 0 (_off + _dlt + 8) (_off + _dlt)) ..10:/#.
+  have->: _off + _dlt + 8 - (_off + _dlt) = 8 by smt().
+  have->: 0 + 0 + (_off + _dlt) = _off + _dlt by smt().
+  rewrite eqseq_cat. rewrite !size_sub /#. move => [#] h0_0 h0_1.
+  rewrite h0_0.
+    rewrite (eq_from_nth W8.zero _ (sub _buf 0 (_off + _dlt))).
+    + rewrite !size_sub /#.
+    + rewrite size_sub 1:/# => i i_bnd.
+      rewrite /l1 !nth_sub ..2:/# initE ifT 1:/# /get8 /set64_direct initE ifT 1:/#.
+      rewrite /= ifF 1:/# initE /#. smt().
+  rewrite (sub_cat result.`1 _off _dlt (min _len 16) 8) ..5:/#.
+  rewrite lez_minl 1:/# h1.
+  have->: take _len (W16u8.to_list _w) =
+          take 8(to_list _w) ++ take (_len-8) (drop 8 (to_list _w))
+          by rewrite -drop_take /#.
+  rewrite set_highu64. congr.
+  move: h0. rewrite !(sub_cat _ 0 0 (_off + _dlt + 8) (_off + _dlt)) ..10:/#.
+  have->: _off + _dlt + 8 - (_off + _dlt) = 8 by smt().
+  have->: 0 + 0 + (_off + _dlt) = _off + _dlt by smt().
+  rewrite eqseq_cat. rewrite !size_sub /#. move => [#] h0_0 h0_1. print set_lowu64.
+  rewrite h0_1 (set_lowu64 _buf _off _dlt _len _w) /#.
+rcondf 1. auto => /#.
+ ecall(a_ilen_write_upto8_at_h buf offset dELTA lEN t64). auto => /> H0 H1 H2 H3 H4 H5 H6. 
+  split; first by smt().
+  rewrite /subwrite_spec =>H7 H8 H9 H10 result _H0 _H1.
+  move: _H0. rewrite /subwrite_pre H7 H8 H9 H10 implyTb => [#]?????.
+  have->: _off + _dlt + 8 - 8 = _off + _dlt by smt().
+  rewrite !lez_minl ..2:/#. move =>  h0 h1 h2 h3.
+  rewrite h2 h3. do split; ..1: smt(); 3..: smt().
+  + rewrite h0 /#.
+  + rewrite h1. 
+    pose l1:= take _len (W8u8.to_list (truncateu64 _w)).
+    pose l2:= take _len (W16u8.to_list _w).
+    rewrite (eq_from_nth W8.zero l1 l2).
+    + rewrite !size_take ..2:/# !size_to_list /#.
+    + rewrite size_take 1:/# size_to_list ifT 1:/#. move => i i_bnd.
+      rewrite !nth_take ..4:/# !nth_to_list /truncateu64 /of_int /to_uint bs2int_mod.
+      rewrite 1:/#. have{1}->:64=size (take 64 (w2bits _w)) 
+        by rewrite size_take 1:/# size_w2bits /#.
+      rewrite bs2intK (W8.ext_eq _ (_w \bits8 i)). move => x x_bnd.
+      + rewrite /(\bits8) !initE !ifT..2:/# /= get_bits2w 1:/# nth_take..2:/#.
+        rewrite get_w2bits /#. smt().
+      smt().
+qed.
+
+phoare a_ilen_write_upto16_at_ph _buf _off _dlt _len _w:
+ [ MM.__a_ilen_write_upto16
+ : buf=_buf /\ offset=_off /\ dELTA=_dlt /\ lEN=_len /\ w = _w /\
+   subwrite_pre _off _dlt _len 16
+ ==> subwriteu128_spec _w 16 _buf _off _dlt _len res.`1 res.`2 res.`3] = 1%r.
+proof.
+by conseq a_ilen_write_upto16_ll
+          (a_ilen_write_upto16_at_h _buf _off _dlt _len _w).
+qed.
+
+op subwriteu256_spec (w : W256.t) (size : int) (_ : W8.t A.t) (off dlt
+  len : int) (buf' : W8.t A.t) (dlt' len' : int) : bool =
+  subwrite_pre off dlt len size =>
+  subwrite_pre off dlt len size /\
+  sub buf' (off + dlt) (min len size) = take len (to_list w) /\
+  dlt' = dlt + min len size /\ len' = max 0 (len - size).
+
+
+lemma u256_from_u256 buf off dlt len size w:
+  size = 32 =>
+  subwrite_pre off dlt len size =>
+  sub (A.init (get8 (set256_direct (WA.init8 (A."_.[_]" buf)) (off + dlt) w))) (off + dlt)
+     (min len 32) =
+  take len (to_list w).
+proof.
+  rewrite /subwriteX_pre => H0 *.
+  + rewrite /sub /to_list -map_take /iotared take_iota minrC.
+    rewrite (eq_in_mkseq _ (((\bits8) w))). move => i i_bnd.
+    + rewrite /get8 /set256_direct /= initE ifT 1:(aux off dlt len _ASIZE i size) ..5:/# /=.
+      rewrite initE ifT 1:(aux off dlt len _ASIZE i size) ..5:/# /= ifT /#. smt().
+qed.
+
+
+lemma set_highu128 _len _w:
+  take (_len - 16) (W16u8.to_list (VEXTRACTI128 _w one)) =
+          take (_len - 16) (drop 16 (to_list _w)).
+proof.
+  move => *.
+  pose l1:= W16u8.to_list (VEXTRACTI128 _w one).
+  pose l2:= drop 16 (W32u8.to_list _w).
+  congr. rewrite (eq_from_nth W8.zero l1 l2).
+  + rewrite size_drop 1:/# !size_to_list /#.
+  + rewrite size_to_list => i i_bnd.
+    rewrite nth_drop ..2:/# /l1 /to_list !nth_to_list_in ..2:/# /VEXTRACTI128.
+    rewrite (W8.ext_eq _ (_w \bits8 16 + i)). move => x x_bnd.
+    + rewrite /(\bits128) /(\bits8) !initE !ifT ..2:/# /= initE ifT 1:/# nth_one /=.
+      rewrite b2i1 /#. smt(). 
+  smt().
+qed.
+
+lemma set_lowu128 buf off dlt len w:
+  0 <= off =>
+  0 <= dlt =>
+  0 <= len =>
+  off + dlt + 16 <= _ASIZE =>
+  sub (A.init (get8 (set128_direct (WA.init8 (A."_.[_]" buf)) (off + dlt) 
+  (truncateu128 w)))) (off + dlt) 16 =
+  take 16 (W32u8.to_list w).
+proof.
+ move =>*.
+ pose l1:= sub (A.init (get8 (set128_direct (WA.init8 ("_.[_]" buf)) (off + dlt) 
+           (truncateu128 w)))) (off + dlt) 16.
+  pose l2:= take 16 (W32u8.to_list w).
+  rewrite (eq_from_nth W8.zero l1 l2).
+  + rewrite size_mkseq size_take 1:/# size_to_list /#.
+  + rewrite size_mkseq lez_maxr 1:/# => i i_bnd.
+    rewrite nth_mkseq 1:/# /= initE ifT 1:/# /get8 /set128_direct.
+    rewrite initE ifT 1:/# /= ifT 1:/# /truncateu128.
+    have->: off + dlt + i - (off + dlt) = i by smt().
+    rewrite nth_take ..2:/# (W8.ext_eq _ (W32u8.to_list w).[i]). move => x x_bnd.
+    + rewrite nth_to_list /(\bits8) !initE !ifT ..2:/# /= /of_int /to_uint.
+      rewrite bs2int_mod 1:/#. 
+      have{1}->:128 = size (take 128 (w2bits w))
+        by rewrite size_take 1:/# size_w2bits /#.
+      rewrite bs2intK get_bits2w 1:/# nth_take ..2:/# get_w2bits /#.
+      smt().
+    smt().
+qed.
+
+hoare a_ilen_write_upto32_at_h _buf _off _dlt _len _w:
+ MM.__a_ilen_write_upto32
+ : buf = _buf /\ offset = _off /\ dELTA = _dlt /\ lEN = _len /\ w = _w /\ 
+   subwrite_pre _off _dlt _len 32 ==>
+   subwriteu256_spec _w 32 _buf _off _dlt _len res.`1 res.`2 res.`3.
+proof.
+proc.
+if => //=; first last.
+auto => /> *. rewrite /subwrite_pre.
+  do split; ..4:smt(); 2..:smt().
+  + rewrite /sub /to_list -map_take /iotared take_iota minrC.
+    rewrite (eq_in_mkseq _ (((\bits8) _w))) /#.
+(*32 <= lEN *)
+if => //=.
+  auto => /> *. do split; ..4:smt();2..: smt(). 
+  rewrite (u256_from_u256 _ _ _ _ 32) /#. 
+sp 1.
+(* 16 <= lEN *)
+case(16 <= lEN). 
+  rcondt 1. auto => /#.
+  ecall(a_ilen_write_upto16_at_h buf offset dELTA lEN t128). 
+  auto => /> H0 H1 H2 H3 H4 H5 H6. 
+  split; first by smt().
+  rewrite /subwriteu128_spec =>H7 H8 H9 H10 result _H0 _H1.
+  move: _H0. rewrite /subwrite_pre H7 H8 H9 H10 implyTb !addrA=> [#]?????.
+  have->: _off + _dlt + 8 - 8 = _off + _dlt by smt().
+  rewrite lez_minl 1:/# => h0 h1 h2 h3.
+  rewrite h2. do split; ..3: smt(); 2..: smt().
+  rewrite (sub_cat result.`1 _off _dlt (min _len 32) 16) ..5:/# lez_minl 1:/# h1.
+  have->: take _len (W32u8.to_list _w) =
+          take 16 (take _len (to_list _w)) ++ take (_len-16) (drop 16 (to_list _w)).
+    rewrite -drop_take 1:/# cat_take_drop /#.
+  rewrite set_highu128. congr.
+  move: h0. rewrite !(sub_cat _ 0 0 (_off + _dlt + 16) (_off + _dlt)) ..10:/#.
+  have->: _off + _dlt + 16 - (_off + _dlt) = 16 by smt().
+  have->: 0 + 0 + (_off + _dlt) = _off + _dlt by smt().
+  rewrite eqseq_cat. rewrite !size_sub /#. move => [#] h0_0 h0_1.
+  rewrite h0_1 take_take (set_lowu128 _buf _off _dlt _len _w) /#.
+rcondf 1. auto => /#.
+  ecall(a_ilen_write_upto16_at_h buf offset dELTA lEN t128). 
+  auto => /> H0 H1 H2 H3 H4 H5 H6. split; first by smt().
+  rewrite /subwriteu128_spec =>H7 H8 H9 H10 result _H0 _H1.
+  move: _H0. rewrite /subwrite_pre H7 H8 H9 H10 implyTb => [#]?????.
+  have->: _off + _dlt + 8 - 8 = _off + _dlt by smt().
+  rewrite !lez_minl ..2:/#. move =>  h0 h1 h2 h3.
+  rewrite h2 h3. do split; ..1: smt(); 2..: smt().
+  rewrite h1.
+  pose l1:= take _len (W16u8.to_list (truncateu128 _w)).
+  pose l2:= take _len (W32u8.to_list _w).
+  rewrite (eq_from_nth W8.zero l1 l2).
+  + rewrite !size_take ..2:/# !size_to_list /#.
+  + rewrite size_take 1:/# size_to_list ifT 1:/#. move => i i_bnd.
+    rewrite !nth_take ..4:/# !nth_to_list /truncateu128 /of_int /to_uint bs2int_mod 1:/#.
+    have{1}->:128 = size (take 128 (w2bits _w)) 
+      by rewrite size_take 1:/# size_w2bits /#.
+    rewrite bs2intK (W8.ext_eq _ (_w \bits8 i)). move => x x_bnd.
+    + rewrite /(\bits8) !initE !ifT..2:/# /= get_bits2w 1:/# nth_take..2:/# get_w2bits /#.
+      smt().
+    smt().
+qed.
+
+phoare a_ilen_write_upto32_at_ph _buf _off _dlt _len _w:
+ [ MM.__a_ilen_write_upto32
+ : buf=_buf /\ offset=_off /\ dELTA=_dlt /\ lEN=_len /\ w = _w /\
+   subwrite_pre _off _dlt _len 32
+ ==> subwriteu256_spec _w 32 _buf _off _dlt _len res.`1 res.`2 res.`3] = 1%r.
+proof.
+by conseq a_ilen_write_upto32_ll
+          (a_ilen_write_upto32_at_h _buf _off _dlt _len _w).
+qed.
+
+*)
 end ReadWriteArray.
